vector+dfs

src/examples/vector.v
@@ -9,33 +9,79 @@ From spacelambda Require Import more_space_lang wp_all triple.
 
 From spacelambda.examples Require Export tactics utils diaframe.
 
-Definition Vector `{!interpGS Σ} (qz : Qz) (qp : Qp) (vs : list val) (l : loc) (capacity : nat) : iProp Σ :=
+(** TODO move *)
+
+Lemma wp_enc_return_unit_iff `{!interpGS Σ} `{Enc A} b t (Q : iProp Σ) :
+  wp_enc b t (λ _ : (), Q) ⊣⊢ wp_enc b t (λ r : val, ⌜r = ()%V⌝ ∗ Q).
+Proof.
+  rewrite !wp_enc_eq /post.
+  apply bi.equiv_entails; split;
+    iIntros "w"; iApply (wp_mono with "w");
+    iIntros (v) "w";
+    iDestruct "w" as ([]) "(-> & q)";
+    iExists val_unit || iExists tt;
+    auto.
+Qed.
+
+Lemma wpc_eq `{!interpGS Σ} `{Enc A} r t Q :
+  wpc r t Q = (∀ k : lctx, ⌜r ⊆ dom k⌝ -∗ Stackables k -∗ wp_enc true t (λ a : A, Stackables k ∗ Q a))%I.
+Proof.
+  reflexivity.
+Qed.
+
+Lemma wps_return_unit_iff `{!interpGS Σ} `{Enc A} X t (Q : iProp Σ) :
+  wps X t (λ _ : (), Q) ⊣⊢ wps X t (λ r : val, ⌜r = ()%V⌝ ∗ Q).
+Proof.
+  rewrite !wps_eq.
+  destruct X. 2: now apply wp_enc_return_unit_iff.
+  rewrite !wpc_eq.
+  apply bi.equiv_entails; split.
+  - iIntros "w" (a) "%Ha Sa".
+    iSpecialize ("w" $! a Ha with "Sa").
+    iApply (wp_enc_mono with "[-]").
+    + iApply wp_enc_return_unit_iff. iApply "w".
+    + iIntros (v) "($ & $ & $)".
+  - iIntros "w" (a) "%Ha Sa".
+    iSpecialize ("w" $! a Ha with "Sa").
+    iApply wp_enc_return_unit_iff.
+    iApply (wp_enc_mono with "[-]").
+    + iApply "w".
+    + iIntros (v) "($ & $ & $)".
+Qed.
+
+Lemma wps_unit_val `{!interpGS Σ} `{Enc A} X t (Q : iProp Σ) :
+  wps X t (λ _ : (), Q) -∗ wps X t (λ _ : val, Q).
+Proof.
+  iIntros "w".
+  iApply (wps_mono with "[w]").
+  iApply (wps_return_unit_iff with "w").
+  iIntros (v) "(_ & $)".
+Qed.
+
+Definition Vector `{!interpGS Σ} (vs : list (val * Qp)) (l : loc) (capacity : nat) : iProp Σ :=
   ∃ (l' : loc),
-    ⌜ length vs <= capacity ⌝
-    ∗ ⌜ 0 < capacity ⌝ (* easier than doing "max 1 n" *)
-    ∗ l ↦ BBlock [ ^capacity; ^(length vs); #l' ]
+    ⌜ length vs <= capacity /\ 0 < capacity ⌝
+    ∗ l ↦ BBlock [ #l'; ^capacity; ^(length vs) ]
     ∗ Stackable l' 1%Qp
-    ∗ l' ↦ BBlock (vs ++ replicate (capacity - length vs) ())
+    ∗ l' ↦ BBlock (vs.*1 ++ replicate (capacity - length vs) ())
     ∗ l' ↤ {[+ l +]}
-    ∗ ([∗ list] v ∈ vs, v ↤?{qz} {[+ l' +]})
-    ∗ ([∗ list] v ∈ vs, vStackable v qp).
+    ∗ ([∗ list] vq ∈ vs, let '(v, q) := vq in vStackable v q ∗ v ↤?{q} {[+ l' +]}).
 
 Definition vector_create : val :=
-  λ: [["n"]],
+  λ: [[]],
     let: "c" := alloc 3 in
-    "c".[0] <- "n" ;;
-    "c".[1] <- ^0 ;;
-    let: "v" := alloc "n" in
-    "c".[2] <- "v" ;;
+    "c".[1] <- ^1 ;;
+    "c".[2] <- ^0 ;;
+    let: "v" := alloc ^1 in
+    "c".[0] <- "v" ;;
     "c".
 
-Lemma vector_create_spec `{!interpGS Σ} (n : nat) qz qp :
-  0 < n ->
-  CODE (vector_create [[^n]])
-  PRE (♢ (3 + n))
-  POST (fun (l:loc) => Vector qz qp [] l n ∗ Stackable l 1%Qp ∗ l ↤ ∅).
+Lemma vector_create_spec `{!interpGS Σ} :
+  CODE (vector_create [[]])
+  PRE (♢ 4)
+  POST (fun (l:loc) => Vector [] l 1 ∗ Stackable l 1%Qp ∗ l ↤ ∅).
 Proof.
-  iIntros (?) "?".
+  iIntros "?".
   wps_call.
   wps_bind. wps_alloc l as "(? & ? & ? & ?)".
   wps_bind. (* Fail wps_store. *) do 7 iStepS.
@@ -44,15 +90,39 @@ Proof.
   wps_bind. wps_store. do 3 iStepS.
   iFrame.
 
-  rew_qz. replace (3 + n - 3 - n)%nat with 0 by lia.
-  iExists l'. rewrite Nat.sub_0_r /= left_id. iFrame.
+  rew_qz.
+  iExists l'. rewrite /= left_id. iFrame.
   iPureIntro; lia.
 Qed.
+
+Definition vector_size : val :=
+  λ: [["p"]],
+    "p".[2].
+
+Lemma vector_size_spec `{!interpGS Σ} vs l cap :
+  CODEFF (vector_size [[#l]])
+  PRE (Vector vs l cap)
+  POST (fun r : nat => ⌜r = length vs⌝ ∗ Vector vs l cap).
+Proof.
+  iIntros "V".
+  iDestruct "V" as (l') "(% & ?)".
+  repeat iStepS.
+Qed.
+
+Parameter time_credit : forall `{!interpGS Σ}, nat -> iProp Σ.
+Notation "$ n" := (time_credit n)%I%Qz (at level 20) : bi_scope.
+
+Parameter time_step_spec : forall `{!interpGS Σ}, forall n m X,
+    triple X
+      ($ (n + m))
+      ("time_step" [[^n]])%T
+      (λ _ : unit, ($ m))%I.
 
 Definition array_copy : val :=
   μ: "self", [["dst", "src", "i", "n"]],
     let: "neq" := "n" '- "i" in
     if: "neq" then
+      "time_step" [[^1]];;
       let: "x" := "src".["i"] in
       "dst".["i"] <- "x";;
       let: "i" := "i" '+ ^1 in
@@ -60,21 +130,32 @@ Definition array_copy : val :=
     else
       ()%V.
 
-Lemma array_copy_spec `{!interpGS Σ} dst src qz src1 src2 src3 dst1 dst3 :
-  qz ≠ 0%Qz ->
+Lemma Qp_not_zero (q : Qp) : (q : Qz) ≠ 0%Qz.
+Proof.
+  assert (0 < Qp_to_Qz q)%Qz as P by now destruct q.
+  intros E; rewrite E in P. revert P.
+  now eapply irreflexivity, StrictOrder_Irreflexive.
+Qed.
+
+Lemma array_copy_spec `{!interpGS Σ} dst src (src1 src2 src3 dst1 dst3 : list (val * Qp)) (time : nat) :
   length src1 = length dst1 ->
   CODE (array_copy [[#dst, #src, ^(length src1), ^(length src1 + length src2)]])
   SOUV {[dst; src]}
-  PRE (src ↦ BBlock (src1 ++ src2 ++ src3)
-     ∗ dst ↦ BBlock (dst1 ++ replicate (length src2) () ++ dst3)
-     ∗ [∗ list] v ∈ src2, v ↤?{qz} {[+ src +]})
-  POST (fun _ =>
-       src ↦ BBlock (src1 ++ src2 ++ src3)
-     ∗ dst ↦ BBlock (dst1 ++ src2 ++ dst3)
-     ∗ [∗ list] v ∈ src2, v ↤?{qz} {[+ src; dst +]}).
+  PRE ($ (length src2 + time)
+     ∗ src ↦ BBlock (src1.*1 ++ src2.*1 ++ src3.*1)
+     ∗ dst ↦ BBlock (dst1.*1 ++ replicate (length src2) () ++ dst3.*1)
+     ∗ [∗ list] vq ∈ src2, let '(v, q) := vq in vStackable v q ∗ v ↤?{q} {[+ src +]})
+  POST (fun _ : () =>
+       $ time
+     ∗ src ↦ BBlock (src1.*1 ++ src2.*1 ++ src3.*1)
+     ∗ dst ↦ BBlock (dst1.*1 ++ src2.*1 ++ dst3.*1)
+     ∗ [∗ list] vq ∈ src2, let '(v, q) := vq in vStackable v q ∗ v ↤?{q} {[+ src; dst +]}).
 Proof.
-  iIntros (Hqz E1).
-  iInduction (src2) as [ | v src2 ] "IH" forall (src1 src3 dst1 dst3 Hqz E1);
+  replace (length dst1) with (length dst1.*1) by rewrite map_length //.
+  replace (length src1) with (length src1.*1) by rewrite map_length //.
+  replace (length src2) with (length src2.*1) by rewrite map_length //.
+  iIntros (E1).
+  iInduction (src2) as [ | (v, q) src2 ] "IH" forall (src1 src3 dst1 dst3 E1);
     iIntros "(? & ? & ?)".
   - wps_call.
     (* we establish that the condition is false *)
@@ -90,13 +171,19 @@ Proof.
     wps_bind. wps_val.
     wps_if. destruct (decide _) as [D|D]. 2:lia.
 
+    (* time step *)
+    wps_bind.
+    wps_apply time_step_spec.
+
     (* loads v *)
     wps_bind.
     unshelve wps_load.
-    { rewrite app_length /=; lia. }
+    { rewrite app_length /= app_length map_length. lia. }
     rewrite list_lookup_total_middle //.
     (* stores v then unit *)
-    wps_bind. unshelve wps_store. by rewrite app_length /=; lia.
+    wps_bind. unshelve wps_store.
+    { rewrite app_length /= !map_length /= app_length /= in E1, D |- *; lia. }
+    { intro; apply Qp_not_zero. }
 
     (* the store introduced some extra vmapsfroms, one of them being for unit *)
     rewrite !list_lookup_total_middle /= //. iClear select True%I.
@@ -105,28 +192,33 @@ Proof.
     wps_bind. wps_val.
 
     (* massaging to match the I.H. *)
-    replace (length src1 + 1) with (length (src1 ++ [v])) by now rewrite app_length /=; lia.
-    replace (length src1 + _) with (length (src1 ++ [v]) + length src2) by now rewrite app_length /=; lia.
-    rewrite insert_app_r_alt /=. 2:lia. replace (_ - _) with O by lia. simpl.
-    rewrite (cons_middle _ dst1) (app_assoc dst1).
-    rewrite (cons_middle _ src1) (app_assoc src1).
-    assert (length (src1 ++ [v]) = length (dst1 ++ [v])) by now rewrite !app_length /=; lia.
+    replace (length src1.*1 + 1) with (length (src1.*1 ++ [v])) by now rewrite app_length map_length /=; lia.
+    replace (length src1.*1 + _) with (length (src1.*1 ++ [v]) + length (src2.*1)) by now rewrite app_length !map_length /=; lia.
+    rewrite insert_app_r_alt /=. 2: rewrite fmap_length in E1, D |- *; lia. rewrite !map_length in E1 |- *. replace (_ - _) with O by lia. simpl.
+    rewrite (cons_middle _ dst1.*1) (app_assoc dst1.*1).
+    rewrite (cons_middle _ src1.*1) (app_assoc src1.*1).
+    assert (length (src1.*1 ++ [v]) = length (dst1.*1 ++ [v])) by now rewrite !app_length !map_length /=; lia.
+    replace (src1.*1 ++ [v]) with (src1 ++ [(v, q)]).*1 by rewrite fmap_app //.
+    replace (dst1.*1 ++ [v]) with (dst1 ++ [(v, q)]).*1 by rewrite fmap_app //.
 
     (* we can finally apply the induction hypothesis -- only thing to be framed is v's mapsfrom *)
     wps_apply "IH"; auto.
-    rewrite -!app_assoc.
+    rewrite !map_length !app_length E1 //.
+    rewrite !fmap_app -!app_assoc.
     iFrame.
+Unshelve. apply tt.
 Qed.
 
 
 Definition vector_resize : val :=
   λ: [["p", "newcap"]],
-    let: "size" := "p".[1] in
-    let: "oldv" := "p".[2] in
+    let: "size" := "p".[2] in
+    let: "oldv" := "p".[0] in
+    "time_step" [["newcap"]];;
     let: "newv" := alloc "newcap" in
     array_copy [["newv", "oldv", ^0, "size"]];;
-    "p".[2] <- "newv";;
-    "p".[0] <- "newcap".
+    "p".[0] <- "newv";;
+    "p".[1] <- "newcap".
 
 Lemma vmapsfroms_cleanup_supd `{!interpGS Σ} b vs l' q ls L:
   ([∗ list] v ∈ vs, v ↤?{q} ls) ∗ †l' =[b | L]=∗
@@ -140,54 +232,70 @@ Proof.
   auto.
 Qed.
 
-Lemma vector_resize_spec `{!interpGS Σ} qz qp vs (oldcap newcap : nat) l :
-  qz ≠ 0%Qz ->
-  oldcap <= newcap ->
+Lemma vmapsfroms_val_Qp_cleanup_supd `{!interpGS Σ} b vs l' ls L:
+  ([∗ list] vq ∈ vs, let '(v,q) := vq in vStackable v q ∗ v ↤?{q} ls) ∗ †l' =[b | L]=∗
+  ([∗ list] vq ∈ vs, let '(v,q) := vq in vStackable v q ∗ v ↤?{q} (ls ⊎ {[-l'-]})).
+Proof.
+  iIntros "(Pvs & #dl)". iIntros (? ? ?) "Hi".
+  iInduction vs as [ | (v, q) vs ] "IH". by auto.
+  simpl big_opL.
+  iDestruct "Pvs" as "((Sv & Pv) & Pvs)".
+  iDestruct (vmapsfrom_cleanup with "[$Pv $dl] Hi") as ">(Hi & $ & _)".
+  iDestruct ("IH" with "Pvs Hi") as ">($ & $)".
+  auto.
+Qed.
+
+Lemma vector_resize_spec `{!interpGS Σ} vs (oldcap newcap : nat) l time :
+  0 < newcap ->
+  length vs <= newcap ->
   CODE (vector_resize [[#l, ^newcap]])
   SOUV {[l]}
-  PRE (Vector qz qp vs l oldcap ∗ ♢newcap)
-  POST (fun _ => Vector qz qp vs l newcap ∗ ♢oldcap).
+  PRE (Vector vs l oldcap ∗ ♢newcap ∗ $ (newcap + (length vs + time)))
+  POST (fun _ : () => Vector vs l newcap ∗ ♢oldcap ∗ $ time).
 Proof.
-  iIntros (Hqz L) "(V & ?)".
-  iDestruct "V" as (l') "(% & % & Hl & Sl' & Hl' & pl' & MP & S)".
+  iIntros (Pnewcap Hnewcap) "(V & ? & ?)".
+  iDestruct "V" as (l') "((%Hlen & %Pcap) & Hl & Sl' & Hl' & pl' & PS)".
   wps_call.
-  wps_bind. wps_load. iIntros.
-  wps_bind. wps_load. iIntros.
+  wps_bind. wps_load.
+  wps_bind. wps_load.
+  wps_bind. wps_apply time_step_spec. iIntros.
   wps_bind. wps_alloc l'' as  "(dia & Hl'' & pl'' & Sl'')".
   iIntros "Sl'".
+  iRename select ($ _)%I into "T".
   iPoseProof
-    (array_copy_spec l'' l' qz nil vs
-       (replicate (oldcap - length vs) ()%V) nil
-       (replicate (newcap - length vs) ()%V)
-      with "[Hl' MP Hl'']") as "A"; auto;
-  [ rewrite -replicate_plus;
+    (array_copy_spec l'' l' nil vs
+       (replicate (oldcap - length vs) (()%V, 1%Qp)) nil
+       (replicate (newcap - length vs) (()%V, 1%Qp)) time
+      with "[Hl' PS Hl'' T]") as "A"; auto;
+  [ rewrite !fmap_replicate -replicate_plus;
     replace (length vs + (newcap - length vs)) with newcap by lia;
     iFrame; auto | ].
 
   wps_bind.
   iApply (wps_context_singleton l'). iFrame.
   iApply (@wps_weak _ _ _ _  {[l''; l']}). now multiset_solver.
+  iApply wps_unit_val.
   iApply (wps_mono with "A").
-  iIntros (_) "(?&?&Pvs) ?".
+  iIntros (_) "(?&?&?&Pvs) ?".
   iIntros "?".
   wps_bind. wps_store.
   assert ({[-l-]} ⊎ {[+l+]} ≡ ∅) as -> by smultiset_solver.
   rew_qz. simpl plus.
   iApply (wps_confront_Stackable l' with "[$]"). iIntros "% ?".
   wps_free l' as "(? & #dl')".
-
-  iApply (wps_esupd _ _ _ _ (vmapsfroms_cleanup_supd true _ l' _ _ _)).
+  rewrite wps_return_unit_iff.
+  iApply (wps_esupd _ _ _ _ (vmapsfroms_val_Qp_cleanup_supd true _ l' _ _)).
   iSplitL "Pvs". by iFrame. iIntros "Pvs".
-  do 6 iStepS.
+  rewrite -wps_return_unit_iff.
+  do 5 iStepS.
   rewrite left_id.
-  rewrite /= app_length replicate_length.
+  rewrite /= app_length !fmap_replicate replicate_length map_length.
   replace (length vs + (oldcap - length vs)) with oldcap by lia.
   iFrame.
   iExists _; iFrame.
   iSplitR. iPureIntro; lia.
-  iSplitR. iPureIntro; lia.
   rewrite big_sepL_proper. iFrame.
-  intros ? ? ?.
+  intros ? (?, ?) ?.
   assert (({[+ l'; l'' +]} ⊎ {[-l'-]} : smultiset _)
             ≡ {[+ l'' +]}) as -> by smultiset_solver.
   auto.
@@ -197,157 +305,233 @@ Qed.
 
 Definition vector_push : val :=
   λ: [["p", "x"]],
-    let: "cap" := "p".[0] in
-    let: "size" := "p".[1] in
+    let: "cap" := "p".[1] in
+    let: "size" := "p".[2] in
     let: "diff" := "cap" '- "size" in
+    "time_step" [[^1]];;
     (if: "diff" then ()%V else
        let: "newcap" := "cap" '* ^2 in
-      vector_resize [["p", "newcap"]]);;
-    let: "v" := "p".[2] in
+       vector_resize [["p", "newcap"]]
+    )%V;;
+    let: "v" := "p".[0] in
     "v".["size"] <- "x";;
     let: "size" := "size" '+ ^1 in
-    "p".[1] <- "size".
+    "p".[2] <- "size".
 
-Lemma vector_push_spec_no_resize `{!interpGS Σ} qz qp vs l v cap :
-  qz ≠ 0%Qz ->
+Lemma vector_push_spec_no_resize `{!interpGS Σ} vs l v (q : Qp) cap time :
   length vs < cap ->
   CODE (vector_push [[#l, v]])
   SOUV {[l]}
-  PRE (vStackable v qp ∗ v ↤?{qz} ∅ ∗ Vector qz qp vs l cap)
-  POST (fun _ => Vector qz qp (vs ++ [v]) l cap).
+  PRE (vStackable v q ∗ v ↤?{q} ∅ ∗ Vector vs l cap ∗ $ (S time))
+  POST (fun _ : () => Vector (vs ++ [(v, q)]) l cap ∗ $ time).
 Proof.
-  iIntros (Hqz Hvs) "(Sv & pv & V)".
-  iDestruct "V" as (l') "(%len & % & Hl & Sl' & Hl' & pl' & pvs & Svs)".
+  iIntros (Hvs) "(Sv & pv & V & T)".
+  iDestruct "V" as (l') "((%Hlen & %Pcap) & Hl & Sl' & Hl' & pl' & PS)".
+  wps_nofree.
   wps_call.
-  wps_bind. wps_load; [ .. | iIntros "Sv"].
-  wps_bind. wps_load; [ .. | iIntros "Sv"].
-  wps_bind. wps_val; [ .. | iIntros "Sv"].
+  wps_bind. wps_load.
+  wps_bind. wps_load.
+  wps_bind. wps_val.
+  wps_bind. wps_apply time_step_spec.
   wps_bind. wps_if. destruct (decide _) as [d|e]. 2:lia.
-  wps_val. iIntros "Sv".
-  wps_bind. wps_load; [ .. | iIntros "Sv"].
+  wps_val.
+  wps_bind. wps_load.
   wps_bind. unshelve wps_store; [ .. | ].
-  now rewrite app_length replicate_length; lia.
+  now rewrite app_length replicate_length map_length; lia.
+  now intro; apply Qp_not_zero.
   wps_bind. wps_val; [ .. | ].
-  do 6 iStepS.
+  do 5 iStepS.
+  iFrame.
   iExists l'.
   rewrite app_length /=.
   iSplitR. now iPureIntro; lia.
-  iSplitR. easy.
   iFrame.
-  rewrite insert_app_r_alt /= // Nat.sub_diag.
+  rewrite insert_app_r_alt map_length /= // Nat.sub_diag.
   replace (cap - length vs) with (1 + (cap - (length vs + 1))) by lia.
-  rewrite -app_assoc /= left_id.
+  rewrite fmap_app -app_assoc /= left_id.
   iFrame.
 Qed.
 
-Lemma vector_push_spec_resize `{!interpGS Σ} qz qp vs l v cap :
-  qz ≠ 0%Qz ->
+Lemma vector_push_spec_resize `{!interpGS Σ} vs l v (q : Qp) cap time :
   length vs = cap ->
   CODE (vector_push [[#l, v]])
   SOUV {[l]}
-  PRE (vStackable v qp ∗ v ↤?{qz} ∅ ∗ Vector qz qp vs l cap ∗ ♢(length vs * 2))
-  POST (fun _ => Vector qz qp (vs ++ [v]) l (cap * 2) ∗ ♢(length vs)).
+  PRE (vStackable v q ∗ v ↤?{q} ∅ ∗ Vector vs l cap ∗ ♢(length vs * 2) ∗ $ (S (length vs * 3 + time)))
+  POST (fun _ : () => Vector (vs ++ [(v, q)]) l (cap * 2) ∗ ♢(length vs) ∗ $ time).
 Proof.
-  iIntros (Hqz Hvs) "(Sv & pv & V & dia)".
-  iDestruct "V" as (l') "(%len & % & Hl & Sl' & Hl' & pl' & pvs & Svs)".
+  iIntros (Hvs) "(Sv & pv & V & dia & T)".
+  iDestruct "V" as (l') "((%Hlen & %Pcap) & Hl & Sl' & Hl' & pl' & PS)".
   wps_call.
   wps_bind. wps_load; [ .. | iIntros "Sv"].
   wps_bind. wps_load; [ .. | iIntros "Sv"].
   wps_bind. wps_val; [ .. | iIntros "Sv"].
+  wps_bind. wps_apply time_step_spec. iIntros "Sv".
   wps_bind. wps_if. destruct (decide _) as [d|e]. lia.
   wps_bind. wps_val.
   assert (length vs <= length vs * 2) as A by lia.
-  wps_apply vector_resize_spec. eassumption. eassumption.
+  replace (length vs * 3 + time)%nat with (length vs * 2 + (length vs + time))%nat by lia.
+  wps_apply vector_resize_spec. lia. eassumption.
   rew_qz. iFrame.
   iSplitR "pv".
   + iExists l'. iFrame.
     iSplitR; auto.
-  + iIntros (_) "(V&?) ?".
-    iDestruct "V" as (l'') "(% & % & Hl & Sl' & Hl' & pl' & pvs & Svs)".
+  + iIntros (_) "(V&?&T) ?".
+    iDestruct "V" as (l'') "((%Hlen' & %Hcap') & Hl & Sl' & Hl' & pl' & PS)".
     wps_bind. wps_load. iIntros "?".
     wps_bind. unshelve wps_store.
-    { rewrite app_length replicate_length. lia. }
+    { rewrite app_length replicate_length map_length. lia. }
+    { intro; apply Qp_not_zero. }
     wps_bind. wps_val.
-    do 6 iStepS.
+    do 5 iStepS.
     iFrame select (♢_)%I.
+    iFrame select ($ _)%I.
     iExists l''.
     rewrite app_length /=.
-    iSplitR. now iPureIntro; lia.
-    iSplitR. easy.
+    iSplitR. iPureIntro; lia.
     iFrame.
-    rewrite insert_app_r_alt /= // Nat.sub_diag.
-    replace (length vs * 2 - length vs) with (1 + (length vs - 1))%nat by lia.
-    replace (length vs * 2 - (length vs + 1)) with (length vs - 1)%nat by lia.
-    rewrite -app_assoc /= left_id.
+    rewrite insert_app_r_alt map_length /= // Nat.sub_diag.
+    replace (length vs * 2 - length vs) with (1 + (length vs - 1)) by lia.
+    replace (length vs * 2 - (length vs + 1)) with (length vs - 1) by lia.
+    rewrite fmap_app -app_assoc /= left_id.
     iFrame.
 Qed.
 
 Definition vector_get : val :=
   λ: [["p", "i"]],
-    let: "v" := "p".[2] in
+    let: "v" := "p".[0] in
     "v".["i"].
 
-Lemma vector_get_spec `{!interpGS Σ} qz qp vs l cap i :
+Lemma vector_get_spec `{!interpGS Σ} vs l cap i :
   i < length vs ->
   CODE (vector_get [[#l, ^i]])
   SOUV {[l]}
-  PRE (Vector qz qp vs l cap)
-  POST (fun r => ⌜r = vs !!! i⌝ ∗ Vector qz qp vs l cap).
+  PRE (Vector vs l cap)
+  POST (fun r => ⌜r = (vs !!! i).1⌝ ∗ Vector vs l cap).
 Proof.
   intros Hi.
   wps_call. iStepS.
   wps_bind. wps_load.
-  unshelve wps_load. by rewrite app_length; lia.
-  iSplitR. iPureIntro. by rewrite lookup_total_app_l //.
+  unshelve wps_load. by rewrite app_length map_length; lia.
+  iSplitR. iPureIntro.
+  rewrite lookup_total_app_l //.
+  now rewrite list_lookup_total_fmap //.
+  now rewrite map_length.
   iExists _. iFrame.
   auto.
 Qed.
 
+(* When a goal is not convertible or equal to an Iris hypothesis
+   ["H" : hyp], use [iExactEq ≡ "H"], which will replace your [goal]
+   with [⌜goal ≡ hyp⌝] *)
+Tactic Notation "iExactEq" "≡" constr(irisHyp) :=
+  match goal with
+  | |- environments.envs_entails ?Δ ?goal =>
+    match Δ with
+    | context[environments.Esnoc _ (INamed irisHyp) ?hyp] =>
+      iAssert ⌜goal ≡ hyp⌝%I as %->; [ | iApply irisHyp ]
+    end
+  end.
+
+(* Same with [=] instead of [≡] *)
+Tactic Notation "iExactEq" "=" constr(irisHyp) :=
+  match goal with
+  | |- environments.envs_entails ?Δ ?goal =>
+    match Δ with
+    | context[environments.Esnoc _ (INamed irisHyp) ?hyp] =>
+      iAssert ⌜goal = hyp⌝%I as %->; [ | iApply irisHyp ]
+    end
+  end.
+
+(** Second spec for [vector_get] which provides a fraction of the
+    stackable/mapsfrom assertions *)
+
+Lemma vector_get_spec_borrow `{!interpGS Σ} vs l cap i :
+  i < length vs ->
+  CODE (vector_get [[#l, ^i]])
+  SOUV {[l]}
+  PRE (Vector vs l cap)
+  POST (fun r =>
+          let '(v, q) := vs !!! i in
+          ⌜r = v⌝
+        ∗ ∀ (q1 q2 : Qp),
+          ⌜(q1 + q2 = q)%Qp⌝ →
+          vStackable v q1
+        ∗ v ↤?{q1} ∅
+        ∗ Vector (<[i := (v, q2)]> vs) l cap
+  ).
+Proof.
+  iIntros (Hi) "V".
+  wps_apply vector_get_spec; auto.
+  iDestruct select _ as "(-> & V)".
+  iDestruct "V" as (l') "((%Hlen & %Pcap) & Hl & Sl' & Hl' & pl' & PS)".
+  destruct (vs !!! i) as (v, q) eqn:Ei. iSplit; auto.
+  iIntros (q1 q2 <-).
+
+  iAssert (vStackable v q1 ∗ v ↤?{q1} ∅
+   ∗ [∗ list] vq ∈ (<[i:=(v, q2)]> vs), let '(v, q) := vq in vStackable v q ∗ v ↤?{q} {[+ l' +]})%I
+    with "[PS]" as "($ & $ & PS)".
+  { iDestruct (big_sepL_insert_acc with "[$]") as "(PS & A)".
+    apply list_lookup_lookup_total_lt; eauto.
+    rewrite Ei. iDestruct "PS" as "((S1 & S2) & P)".
+    iAssert (v ↤?{q1 + q2} (∅ ⊎ {[+ l' +]}))%I with "[P]" as "P".
+    by rewrite left_id -Qp_to_Qz_plus_distr //.
+    iDestruct (vmapsfrom_split with "P") as "(P1 & P2)".
+    1,2 : by intros; edestruct Qp_not_zero; eauto.
+    iFrame. iApply "A"; iFrame. }
+
+  iExists _.
+  rewrite insert_length.
+  iFrame.
+  iSplit; auto.
+  iExactEq = "Hl'". iPureIntro. do 3 f_equal.
+  apply list_eq; intros j.
+  rewrite !list_lookup_fmap.
+  destruct (decide (i = j)) as [<- | n].
+  - rewrite !list_lookup_insert /= // list_lookup_lookup_total_lt /= // Ei //.
+  - rewrite !list_lookup_insert_ne //.
+Qed.
+
 Definition vector_set : val :=
   λ: [["p", "i", "x"]],
-    let: "v" := "p".[2] in
+    let: "v" := "p".[0] in
     "v".["i"] <- "x".
 
-Lemma vector_set_spec `{!interpGS Σ} qz qp vs l cap i (x : val) :
-  qz ≠ 0%Qz ->
+Lemma vector_set_spec `{!interpGS Σ} vs l cap i (x : val) (q : Qp) :
   i < length vs ->
   CODE (vector_set [[#l, ^i, x]])
   SOUV {[l]}
-  PRE (vStackable x qp
-     ∗ x ↤?{qz} ∅
-     ∗ Vector qz qp vs l cap)
-  POST (fun r =>
-       vStackable (vs !!! i) qp
-     ∗ (vs !!! i) ↤?{qz} ∅
-     ∗ Vector qz qp (<[i:=x]> vs) l cap).
+  PRE (vStackable x q
+     ∗ x ↤?{q} ∅
+     ∗ Vector vs l cap)
+  POST (fun _ : () =>
+       (let '(v,q) := vs !!! i in vStackable v q ∗ v ↤?{q} ∅ )
+     ∗ Vector (<[i:=(x, q)]> vs) l cap).
 Proof.
-  intros Hqz Hi.
-  iIntros "(? & ? & V)".
-  iDestruct "V" as (l') "(% & % & ? & ? & ? & ? & Pvs & Svs)".
+  intros Hi.
+  iIntros "(Sx & ? & V)".
+  iDestruct "V" as (l') "((%Hlen & %Pcap) & ? & ? & ? & ? & PS)".
+  wps_nofree.
   wps_call.
-  wps_bind. wps_load. iIntros "Sx".
-  unshelve (do 4 iStepS). by rewrite app_length; lia.
+  wps_bind. wps_load.
+  unshelve (do 3 iStepS). by rewrite app_length map_length; lia.
 
-  iAssert (vStackable (vs !!! i) qp ∗
-    [∗ list] v ∈ (<[i:=x]> vs), vStackable v qp)%I
-    with "[Sx Svs]" as "(Sv & Svs)".
-  { iDestruct (big_sepL_insert_acc with "[$]") as "($ & A)".
-    apply list_lookup_lookup_total_lt; auto.
-    iApply "A"; auto. }
+  destruct (vs !!! i) as (v_, q_) eqn:Ei.
 
-  iExists qz, ∅. iFrame.
-  iSplitR. iPureIntro; auto.
+  iExists q, ∅. iFrame.
+  iSplitR. iPureIntro; intro; apply Qp_not_zero.
   iIntros (_) "(? & Px & Pv)".
 
-  iAssert ((vs !!! i) ↤?{qz} {[+ l' +]}∗
-    [∗ list] v ∈ <[i:=x]> vs, v ↤?{qz} {[+ l' +]})%I
-    with "[Px Pvs]" as "(Pv2 & Pvs)".
-  { rewrite left_id.
-    iDestruct (big_sepL_insert_acc with "[$]") as "($ & A)".
+  iAssert (vStackable v_ q_ ∗ v_ ↤?{q_} {[+ l' +]} ∗
+    [∗ list] vq ∈ (<[i:=(x, q)]> vs), let '(v,q) := vq in vStackable v q ∗ v ↤?{q} {[+ l' +]})%I
+    with "[Px Sx PS]" as "(Sv_ & Pv_ & PS)".
+  { iDestruct (big_sepL_insert_acc with "[$]") as "(PS & A)".
     apply list_lookup_lookup_total_lt; eauto.
-    iApply "A"; auto. }
+    rewrite Ei. iDestruct "PS" as "($ & $)".
+    rewrite left_id.
+    iApply "A"; iFrame. }
 
-  rewrite lookup_total_app_l /= //.
+  rewrite lookup_total_app_l /= // ?map_length //.
+  rewrite list_lookup_total_fmap // Ei /=.
   iDestruct (vmapsfrom_join with "[$]") as "?".
 
   assert ({[+ l' +]} ⊎ {[-l'-]} ≡ (∅ : smultiset _)) as -> by smultiset_solver.
@@ -355,83 +539,218 @@ Proof.
   iFrame.
 
   iExists l'. iFrame.
-  rewrite insert_length insert_app_l /= //.
+  rewrite insert_length insert_app_l /= ?map_length // list_fmap_insert.
   iFrame. auto.
 Qed.
 
 Definition vector_pop : val :=
   λ: [["p"]],
-    let: "v" := "p".[2] in
-    let: "size" := "p".[1] in
+    let: "v" := "p".[0] in
+    let: "cap" := "p".[1] in
+    let: "size" := "p".[2] in
     let: "size" := "size" '- ^1 in
     let: "x" := "v".["size"] in
-    "p".[1] <- "size";;
+    "time_step" [[^1]];;
     "v".["size"] <- ();;
+    "p".[2] <- "size";;
+    let: "size_times_4" := "size" '* ^4 in
+    let: "cap_small_enough" := "size_times_4" '- "cap" in
+    (if: "cap_small_enough" then ()%V else
+      let: "newcap" := if: "size" then "size" '* ^2 else (^1)%V in
+      vector_resize [["p", "newcap"]]
+    );;
     "x".
 
-Lemma diamonds_le `{!interpGS Σ} n m : n <= m -> ♢ m -∗ ♢ n.
-Proof.
-  intros.
-  replace m with (n + (m - n)) by lia.
-  rewrite nat_to_Qz_add diamond_split_iff.
-  iIntros "($ & ?)".
-Qed.
-
-Lemma vector_pop_spec `{!interpGS Σ} qz qp vs l cap (x : val) :
-  qz ≠ 0%Qz ->
+Lemma vector_pop_spec_no_resize `{!interpGS Σ} vs l cap (x : val) (q : Qp) time :
+  cap < 4 * length vs ->
   CODE (vector_pop [[#l]])
   SOUV {[l]}
-  PRE (Vector qz qp (vs ++ [x]) l cap)
+  PRE (Vector (vs ++ [(x, q)]) l cap ∗ $ (S time))
   POST (fun r => ⌜r = x⌝
-      ∗ vStackable x qp
-      ∗ x ↤?{qz} ∅
-      ∗ Vector qz qp vs l cap).
+      ∗ vStackable x q
+      ∗ x ↤?{q} ∅
+      ∗ Vector vs l cap
+      ∗ $ time).
 Proof.
-  intros Hqz.
-  iIntros "V".
-  iDestruct "V" as (l') "(% & % & ? & ? & ? & ? & Pvs & Svs)".
+  iIntros (Hcap) "(V & T)".
+  iDestruct "V" as (l') "((%Hlen & %Pcap) & ? & ? & ? & ? & PS)".
+  wps_nofree.
+  wps_call.
+  wps_bind. wps_load.
+  wps_bind. wps_load.
+  wps_bind. wps_load.
+  wps_bind. wps_val.
+  wps_bind. wps_load.
+  wps_bind. wps_apply time_step_spec.
+  rewrite fmap_app -app_assoc list_lookup_total_middle ?app_length ?map_length /= //. 2:lia.
+  rewrite !big_opL_snoc.
+  iDestruct "PS" as "(PS & Sx & Px)".
+  wps_bind. wps_store.
+  wps_bind. wps_store.
+  wps_bind. wps_val.
+  wps_bind. wps_val.
+  wps_bind. wps_if.
+  destruct (decide _) as [i|i]; rewrite app_length /= in Hlen, i |- *. 2:lia.
+  wps_val.
+  rewrite list_lookup_total_middle ?app_length ?map_length /= //. 2:lia.
+  iDestruct (vmapsfrom_join with "[$]") as "Px".
+  assert ({[- l' -]} ⊎ {[+l'+]} ≡ (∅ : smultiset _)) as -> by smultiset_solver.
+  rewrite left_id.
+  wps_val. iSplitR; auto. iFrame "Sx Px".
+  replace (length vs + 1 - 1) with (length vs) by lia.
+  iFrame.
+  iExists l'. iFrame.
+  iStepS.
+  set (b1 := BBlock _); set (b2 := BBlock _); assert (b1 = b2) as ->; auto. subst b1 b2; f_equal.
+  rewrite insert_app_r_alt map_length // Nat.sub_diag /= -replicate_S. do 2 f_equal.
+  lia.
+Unshelve.
+  rewrite !app_length map_length app_length /=. lia.
+  rewrite !app_length map_length /=. lia.
+Qed.
+
+(** Transforms the goal [if C then wps X t1 Q else wps X t2 Q]
+  into [Q (if C then v1 else v2)]
+  if [t1] and [t2] can be proved to evaluate to [v1] and [v2] *)
+
+Ltac wps_if_val v1 v2 :=
+  match goal with
+    |- environments.envs_entails ?E (if decide ?C then wps ?X ?t1 ?Q else wps ?X ?t2 ?Q) =>
+      cut (environments.envs_entails E (Q (if decide C then v1 else v2)));
+      [ destruct (decide C); intro; wps_val; assumption | ]
+  end.
+
+(** Transforms [if C then (f A) else (f B)] into [f (if C then A else B)] *)
+
+Ltac fold_if :=
+  match goal with
+    |- context[if ?C then (?f ?A) else (?f ?B)] =>
+      replace (if C then (f A) else (f B))
+      with (f (if C then A else B))
+      by now destruct C
+  end.
+
+Lemma vector_pop_spec_resize `{!interpGS Σ} vs l cap (x : val) (q : Qp) time :
+  cap >= 4 * length vs ->
+  CODE (vector_pop [[#l]])
+  SOUV {[l]}
+  PRE (Vector (vs ++ [(x, q)]) l cap
+      ∗ ♢(1 `max` (length vs * 2))%nat
+      ∗ $ (S (1 `max` (length vs * 2)) + (length vs + time)))
+  POST (fun r => ⌜r = x⌝
+      ∗ vStackable x q
+      ∗ x ↤?{q} ∅
+      ∗ Vector vs l (1 `max` (length vs * 2))
+      ∗ ♢cap
+      ∗ $ time).
+Proof.
+  iIntros (Hcap) "(V & dia & T)".
+  iDestruct "V" as (l') "((%Hlen & %Pcap) & ? & ? & ? & ? & PS)".
   wps_call.
   wps_bind. wps_load.
   wps_bind. wps_load. iIntros "?".
+  wps_bind. wps_load. iIntros "?".
   wps_bind. wps_val. iIntros "?".
-  wps_bind. wps_store.
-  rewrite !big_opL_snoc app_length /= Nat.add_sub.
-  rewrite -app_assoc list_lookup_total_middle //.
-  iDestruct "Pvs" as "(Pvs & Px)".
-  iDestruct "Svs" as "(Svs & Sx)".
+  wps_bind. wps_load. iIntros "?".
+  rewrite fmap_app -app_assoc list_lookup_total_middle ?app_length ?map_length /= //. 2:lia.
+  rewrite !big_opL_snoc.
+  iDestruct "PS" as "(PS & Sx & Px)".
+  replace (length vs + 1 - 1) with (length vs) by lia.
+  wps_bind. wps_apply time_step_spec. iIntros.
+  wps_bind. Fail wps_store. do 7 iStepS.
+  wps_bind. Fail wps_store. do 7 iStepS.
+  wps_bind. wps_val. iIntros "?".
+  wps_bind. wps_val. iIntros "?".
+  wps_bind. wps_if.
+  destruct (decide _) as [i|i]; rewrite app_length /= in Hlen, i |- *. lia.
+  wps_bind. wps_if.
 
-  wps_bind. wps_store.
-  wps_bind. wps_store.
-  rewrite list_lookup_total_middle //.
-  iDestruct (vmapsfrom_join with "[$]") as "?".
+  wps_if_val (length vs * 2)%V 1%V.
+  rewrite insert_app_r_alt; rewrite map_length//.
+  rewrite Nat.sub_diag /= -replicate_S.
+  replace (S (cap - (length vs + 1))) with (cap - length vs) by lia.
+  fold_if.
+
+  wps_apply (vector_resize_spec vs). 1,2: destruct vs; simpl; lia.
+  rewrite list_lookup_total_middle ?app_length ?map_length /= //.
+  iDestruct (vmapsfrom_join with "[$]") as "Px".
   assert ({[- l' -]} ⊎ {[+l'+]} ≡ (∅ : smultiset _)) as -> by smultiset_solver.
   rewrite left_id.
-  iStepS.
-  iStepS.
-  iStepS.
-  iStepS.
-
-  iExists l'. iFrame.
-  iStepS.
-  iStepS.
-  set (b1 := BBlock _); set (b2 := BBlock _); assert (b1 = b2) as ->; auto. subst b1 b2; f_equal.
-  rewrite insert_app_r_alt // Nat.sub_diag /= -replicate_S. do 2 f_equal.
-  rewrite ->app_length in *. simpl in *. lia.
+  rew_qz.
+  assert (1 `max` (length vs * 2) = if decide (length vs ≠ 0) then (length vs * 2) else 1)%nat
+     as E by (destruct (decide _) as [h|h]; lia).
+  rewrite -E.
+  iFrame.
+  iSplitR "Px".
+  { iFrame. iExists l'. iFrame. iPureIntro; lia. }
+  iIntros (_) "(V&?) Sx".
+  iDestruct "V" as (l'') "((%Hlen' & %Pcap') & Hl & Sl' & Hl' & pl' & PS)".
+  wps_val. iSplitR; auto. iFrame.
+  iExists l''. iFrame. auto.
 Unshelve.
-  rewrite !app_length /=. lia.
-  rewrite !app_length /=. lia.
-  rewrite ->app_length in *. simpl in *. lia.
+  rewrite !app_length map_length app_length /=. lia.
+  rewrite !app_length map_length /=. lia.
 Qed.
 
-Lemma vector_free `{!interpGS Σ} qz qp vs l cap :
-  Stackable l 1%Qp ∗ l ↤ ∅ ∗ Vector qz qp vs l cap =#=∗
+Lemma vector_pop_joined_specs `{!interpGS Σ} vs l cap (x : val) (q : Qp) time :
+  let cond := decide (4 * length vs <= cap) in
+  let newcap := 1 `max` (length vs * 2) in
+  CODE (vector_pop [[#l]])
+  SOUV {[l]}
+  PRE (Vector (vs ++ [(x, q)]) l cap
+      ∗ (if cond then ♢newcap else True)
+      ∗ $ (if cond then S (1 `max` (length vs * 2)) + (length vs + time) else S time)%nat)
+  POST (fun r => ⌜r = x⌝
+      ∗ vStackable x q
+      ∗ x ↤?{q} ∅
+      ∗ Vector vs l (if cond then newcap else cap)
+      ∗ (if cond then ♢cap else True)
+      ∗ $ time).
+Proof.
+  destruct (decide _).
+  - apply vector_pop_spec_resize; auto.
+  - iIntros "(V & ? & ?)". wps_apply vector_pop_spec_no_resize. lia. iFrame.
+Qed.
+
+Lemma vector_pop_joined_specs_lookup `{!interpGS Σ} vs l cap time :
+  vs ≠ [] ->
+  let cond := decide (4 * (length vs - 1) <= cap) in
+  let newcap := 1 `max` ((length vs - 1) * 2) in
+  CODE (vector_pop [[#l]])
+  SOUV {[l]}
+  PRE (Vector vs l cap
+      ∗ (if cond then ♢newcap else True)
+      ∗ $ (if cond then S newcap + (length vs - 1 + time) else S time)%nat)
+  POST (fun r =>
+        let '(x, q) := vs !!! (length vs - 1) in
+        ⌜r = x⌝
+      ∗ vStackable x q
+      ∗ x ↤?{q} ∅
+      ∗ Vector (rev (tail (rev vs))) l (if cond then newcap else cap)
+      ∗ (if cond then ♢cap else True)
+      ∗ $ time).
+Proof.
+  intros Hvs.
+  rewrite -(rev_involutive vs) in Hvs |- *.
+  destruct (rev vs) as [ | (x, q) ? ]. tauto.
+  iIntros "(V & d & T)".
+  simpl rev.
+  rewrite list_lookup_total_middle ?app_length ?Nat.add_sub //.
+  wps_apply (vector_pop_joined_specs (rev l0) l cap x q).
+  rewrite rev_app_distr /= rev_involutive //.
+Qed.
+
+(** note: here, but already in the pop/push specifications with resize, time for
+    freeing and garbage collection was not accounted for. *)
+
+Lemma vector_free `{!interpGS Σ} vs l cap :
+  Stackable l 1%Qp ∗ l ↤ ∅ ∗ Vector vs l cap =#=∗
   ♢(cap + 3) ∗ †l
-    ∗ ([∗ list] v ∈ vs, v ↤?{qz} ∅)
-    ∗ ([∗ list] v ∈ vs, vStackable v qp).
+  ∗ ([∗ list] vq ∈ vs, let '(v,q) := vq in vStackable v q ∗ v ↤?{q} ∅).
 Proof.
   iIntros "(Sl & Pl & V)".
   iIntros (? ? ?) "I".
-  iDestruct "V" as (l') "(%len & % & Hl & Sl' & Hl' & pl' & pvs & Svs)".
+  iDestruct "V" as (l') "((%Hlen & %Pcap) & Hl & Sl' & Hl' & pl' & PS)".
   iMod (@interp_free _ _ _ k σ _ ∅ l with "[$]") as "(Hi & ? & #dl)".
   { set_solver. }
   { set_solver. }
@@ -441,22 +760,33 @@ Proof.
   { set_solver. }
   { set_solver. }
   iDestruct (diamonds_join with "[$]") as "dia".
-  rewrite /size_block app_length replicate_length. simpl length. rew_qz.
+  rewrite /size_block app_length replicate_length map_length. simpl length. rew_qz.
   replace (length vs + (cap - length vs) + 3) with (cap + 3) by lia.
-  iFrame "Svs dia dl".
-  clear len.
+  iFrame "dia dl".
+  clear Hlen.
 
-  iPoseProof (vmapsfroms_cleanup_supd true _ l' _ {[+ l' +]} _ with "[$] Hi")
+  iPoseProof (vmapsfroms_val_Qp_cleanup_supd true _ l' _ {[+ l' +]} with "[$] Hi")
     as ">($ & Pvs)".
   rewrite big_sepL_proper. auto.
-  intros ? ? ?. rewrite -opposite_singleton opposite_cancel //.
+  intros ? (?, ?) ?. rewrite -opposite_singleton opposite_cancel //.
 Qed.
 
-Ltac gather_diamonds := repeat (iDestruct (diamonds_join with "[$]") as "?"; rew_qz; simpl Nat.add).
+(** Cleanup tactic for proving examples *)
+
+Import environments.
+Local Ltac cleanup :=
+  simpl;
+  repeat (
+      match goal with |- envs_entails _ (_ -∗ _) => iIntros "?" end
+     || match goal with |- envs_entails _ (∀ _, _) => iIntros (?) end
+     || match goal with |- envs_entails _ (♢ ?n ∗ _)%I => mine n as "_H"; [ iFrame "_H" | ..] end
+     || iDestruct (diamonds_join with "[$]") as "?"
+     || iDestruct select (_ ∗ _)%I as "(? & ?)"
+     || iDestruct select (⌜_⌝)%I as "%").
 
 Example example `{!interpGS Σ} :
   CODE (
-      let: "v" := vector_create [[^1]] in
+      let: "v" := vector_create [[]] in
       vector_push [["v", ^1]];;
       vector_push [["v", ^2]];;
       vector_push [["v", ^3]];;
@@ -470,160 +800,351 @@ Example example `{!interpGS Σ} :
       vector_pop [["v"]];;
       vector_pop [["v"]];;
       vector_pop [["v"]];;
+      vector_pop [["v"]];;
+      vector_pop [["v"]];;
       let: "x" := vector_pop [["v"]] in
       "x"
     )
-  PRE (♢19)
-  POST (fun res : val => ⌜res = 4⌝ ∗ ♢19).
+  PRE (♢19 ∗ $43)
+  POST (fun res : val => ⌜res = 22⌝ ∗ ♢19 ∗ $0).
 Proof.
   iIntros "?".
-  mine 4. wps_bind. wps_apply (vector_create_spec 1 1 1). auto. rew_qz. iStepS. iIntros (l) "(V & S & Pl)".
-  wps_bind. wps_apply vector_push_spec_no_resize; auto. iIntros "?".
-  mine 2.
-  wps_bind. wps_apply vector_push_spec_resize; auto. rew_qz. simpl. iFrame. iIntros (_) "(? & ?) ?".
-  gather_diamonds. mine 4.
-  wps_bind. wps_apply vector_push_spec_resize; auto. rew_qz. simpl. iFrame. iIntros (_) "(? & ?) ?".
-  wps_bind. wps_apply vector_push_spec_no_resize; auto. iIntros "?".
-  gather_diamonds. mine 8.
-  wps_bind. wps_apply vector_push_spec_resize; auto. rew_qz. simpl. iFrame. iIntros (_) "(? & ?) ?".
-  wps_bind. wps_apply vector_push_spec_no_resize. auto. auto. iIntros "?".
-  wps_bind. wps_apply vector_push_spec_no_resize. auto. auto. iIntros "?".
-  wps_bind. wps_apply vector_set_spec. auto. simpl; lia. iIntros "?".
-  wps_bind. wps_apply vector_set_spec. auto. simpl; lia. iIntros "?".
-  wps_bind. wps_apply vector_set_spec. auto. simpl; lia. iIntros "?".
-  repeat iDestruct select (_ ∗ _)%I as "(? & ?)".
-  wps_bind. wps_apply (vector_pop_spec 1 1 [(^11)%V; (^22)%V; (^3)%V; (^4)%V; (^5)%V; (^6)%V] l). auto. iIntros "?".
-  iDestruct select (_ ∗ _)%I as "(-> & % & % & ?)".
-  wps_bind. wps_apply (vector_pop_spec 1 1 [(^11)%V; (^22)%V; (^3)%V; (^4)%V; (^5)%V] l). auto. iIntros "?".
-  iDestruct select (_ ∗ _)%I as "(-> & % & % & ?)".
-  wps_bind. wps_apply (vector_pop_spec 1 1 [(^11)%V; (^22)%V; (^3)%V; (^4)%V] l). auto. iIntros "?".
-  iDestruct select (_ ∗ _)%I as "(-> & % & % & ?)".
+  cleanup.
+  wps_bind. wps_apply vector_create_spec. cleanup.
+  wps_bind. wps_apply vector_push_spec_no_resize; auto. cleanup.
+  wps_bind. wps_apply vector_push_spec_resize; auto. simpl. cleanup.
+  wps_bind. wps_apply vector_push_spec_resize; auto. simpl. cleanup.
+  wps_bind. wps_apply vector_push_spec_no_resize; auto. cleanup.
+  wps_bind. wps_apply vector_push_spec_resize; auto. simpl. cleanup.
+  wps_bind. wps_apply vector_push_spec_no_resize; auto. cleanup.
+  wps_bind. wps_apply vector_push_spec_no_resize; auto. cleanup.
+  wps_bind. wps_apply vector_set_spec; auto. simpl; lia. cleanup.
+  wps_bind. wps_apply vector_set_spec; auto. simpl; lia. cleanup.
+  wps_bind. wps_apply vector_set_spec; auto. simpl; lia. cleanup.
+  wps_bind. wps_apply vector_pop_joined_specs_lookup; auto. cleanup.
+  wps_bind. wps_apply vector_pop_joined_specs_lookup; auto. cleanup.
+  wps_bind. wps_apply vector_pop_joined_specs_lookup; auto. cleanup.
+  wps_bind. wps_apply vector_pop_joined_specs_lookup; auto. cleanup.
+  wps_bind. wps_apply vector_pop_joined_specs_lookup; auto. cleanup.
   wps_bind.
-  iApply (wps_context_singleton l). iFrame.
-  wps_apply (vector_pop_spec 1 1 [(^11)%V; (^22)%V; (^3)%V] l). auto. iIntros "?".
-  iDestruct select (_ ∗ _)%I as "(-> & % & % & ?)".
-  iApply (wps_esupd _ _ _ _ (vector_free 1 1 [(^11)%V; (^22)%V; (^3)%V] l 8) with "[-]").
-  iFrame. iIntros "(? & ? & ? & ? & ?)".
-  gather_diamonds.
-  subst. wps_val. auto.
-  Unshelve.
+  iApply wps_context_singleton. iFrame.
+  wps_apply vector_pop_joined_specs_lookup; auto. cleanup.
+  iApply (wps_esupd _ _ _ _ (vector_free _ _ _)). iFrame. cleanup.
+  subst. wps_val. iSplit; auto. rew_qz; auto. iFrame.
+Unshelve.
+  all: try exact 1%Qp.
   set_solver.
 Qed.
 
-(** Amortized *)
+(** Amortized specifications *)
 
-Definition VectorAm `{!interpGS Σ} (qz : Qz) (qp : Qp) (vs : list val) (l : loc) : iProp Σ :=
-  ∃ (capacity : nat),
-    ♢ (length vs * 3 - capacity)%nat
-    ∗ Vector qz qp vs l capacity.
+Parameter time_credit_join : forall `{!interpGS Σ} (n m : nat),
+  ($ n ∗ $ m -∗ $ (n + m)).
 
-Lemma vector_create_amortized_spec `{!interpGS Σ} (n : nat) qz qp :
-  0 < n ->
-  CODE (vector_create [[^n]])
-  PRE (♢ (3 + n))
-  POST (fun (l:loc) => VectorAm qz qp [] l ∗ Stackable l 1%Qp ∗ l ↤ ∅).
+Parameter time_credit_split : forall `{!interpGS Σ} (n m : nat),
+  ($ (n + m) -∗ $ n ∗ $ m).
+
+Lemma time_credit_split_alt `{!interpGS Σ} (n m : nat) :
+  n <= m -> ($ m -∗ ($ n ∗ $ (m - n))).
 Proof.
-  iIntros (?) "dia".
-  iApply wps_bupd. iMod diamonds_zero. iModIntro.
-  iPoseProof (vector_create_spec n qz qp with "dia") as "A"; auto.
-  iApply (wps_mono with "A").
-  iIntros (l) "(V & $ & $)".
-  iExists n; auto.
+  iIntros (L) "T".
+  replace m with (n + (m - n)) at 1 by lia.
+  iDestruct (time_credit_split with "T") as "($ & $)".
 Qed.
 
-Lemma vector_push_amortized_spec `{!interpGS Σ} qz qp vs l v :
-  qz ≠ 0%Qz ->
+Lemma time_credit_weak `{!interpGS Σ} (n m : nat) :
+  n <= m -> ($ m -∗ $ n).
+Proof.
+  iIntros (L) "T". replace m with (n + (m - n)) by lia.
+  iDestruct (time_credit_split with "T") as "($ & _)".
+Qed.
+
+Definition time_reserve (cap size : nat) : nat :=
+  if decide (cap / 2 <= size) then
+    (size - cap / 2) * 6
+  else
+    (cap / 2 - size) * 3.
+
+Definition VectorAm `{!interpGS Σ} (vs : list (val * Qp)) (l : loc) : iProp Σ :=
+  ∃ (capacity : nat),
+      ⌜ capacity <= 1 `max` (4 * length vs) ⌝
+    ∗ ♢ (1 + length vs * 6 - capacity)%nat
+    ∗ $ (time_reserve capacity (length vs))
+    ∗ Vector vs l capacity.
+
+Lemma vector_create_amortized_spec `{!interpGS Σ} :
+  CODE (vector_create [[]])
+  PRE (♢ 4 ∗ $ 0)
+  POST (fun (l:loc) => VectorAm [] l ∗ Stackable l 1%Qp ∗ l ↤ ∅).
+Proof.
+  iIntros "(Hdiams & T)".
+  mine 4%nat as "dia".
+  iPoseProof (vector_create_spec with "[dia]") as "A"; rew_qz; auto.
+  iApply (wps_mono with "A").
+  iDestruct (time_credit_split 0 with "[$]") as "(T0 & T)".
+  iIntros (l) "(V & $ & $)".
+  iFrame.
+  iExists _; iFrame; simpl; auto.
+Qed.
+
+Lemma vector_size_amortized_spec `{!interpGS Σ} vs l :
+  CODEFF (vector_size [[#l]])
+  PRE (VectorAm vs l)
+  POST (fun r : nat => ⌜r = length vs⌝ ∗ VectorAm vs l).
+Proof.
+  iIntros "V".
+  iDestruct "V" as (l') "(? & ? & ? & V)".
+  iPoseProof (vector_size_spec with "V") as "A".
+  iApply (wps_mono with "A").
+  iIntros (l'') "($ & ?)".
+  iExists _; iFrame.
+Qed.
+
+Lemma vector_push_amortized_spec `{!interpGS Σ} vs l v (q : Qp) :
   CODE (vector_push [[#l, v]])
   SOUV {[l]}
-  PRE (vStackable v qp ∗ v ↤?{qz} ∅ ∗ VectorAm qz qp vs l ∗ ♢3)
-  POST (fun _ => VectorAm qz qp (vs ++ [v]) l).
+  PRE (vStackable v q ∗ v ↤?{q} ∅ ∗ VectorAm vs l ∗ ♢6 ∗ $7)
+  POST (fun _ : () => VectorAm (vs ++ [(v, q)]) l).
 Proof.
-  iIntros (Hqz) "(Sv & pv & V & dia)".
-  iDestruct "V" as (cap) "(dn & V)".
-  destruct (decide (length vs < cap)).
-  - iPoseProof (vector_push_spec_no_resize qz with "[$]") as "A"; auto.
-    iApply (wps_mono with "A"). iIntros (_) "V".
-    iExists cap. iFrame. gather_diamonds. iApply (diamonds_le with "[$]").
-    rewrite app_length /= //. lia.
-  - iAssert ⌜length vs ≤ cap⌝%I as "%". by iDestruct "V" as (?) "($ & ?)".
+  iIntros "(Sv & pv & V & dia & T)".
+  iDestruct "V" as (cap) "(%Ucap & dn & dT & V)".
+  destruct (decide (length vs < cap)) as [ok|over].
+  - iPoseProof (vector_push_spec_no_resize with "[$]") as "A"; auto.
+    iApply (wps_mono with "A"). iIntros (_) "(V & T)".
+    iExists cap. iFrame.
+    iDestruct (time_credit_join with "[$]") as "T".
+    rewrite app_length //.
+    iSplitR.
+    + iPureIntro. lia.
+    + iSplitR "T".
+      * iDestruct (diamonds_join with "[$]") as "?". iApply (diamonds_eq with "[$]"). rew_qz. simpl. lia.
+      * iApply (time_credit_weak with "T"). simpl length.
+        unfold time_reserve. do 2 destruct (decide _); lia.
+  - iAssert ⌜length vs ≤ cap⌝%I as "%". by iDestruct "V" as (?) "(($ & _) & _ & _)".
     assert (cap = length vs) as -> by lia.
-    replace (length vs * 3 - length vs) with (length vs * 2) by lia.
-    iPoseProof (vector_push_spec_resize qz with "[$Sv $pv $V dn]") as "A"; auto. by rew_qz.
-    iApply (wps_mono with "A"). iIntros (_) "(V & d)".
-    iExists (length vs * 2). iFrame. gather_diamonds. iApply (diamonds_le with "[$]").
-    rewrite app_length /= //. lia.
+    iDestruct (diamonds_join with "[$]") as "?".
+    mine (length vs * 2) as "d2".
+    iDestruct (time_credit_join with "[$]") as "T".
+    iDestruct (time_credit_split_alt (S (length vs * 3 + 0)) with "[$]") as "(T1 & T)".
+    { unfold time_reserve.
+      pose proof Nat.div_mod_eq (length vs) 2.
+      pose proof Nat.mod_upper_bound (length vs) 2.
+      destruct (decide _); lia. }
+    iPoseProof (vector_push_spec_resize with "[$Sv $pv $V d2 $T1]") as "A"; auto. by rew_qz.
+    iApply (wps_mono with "A"). iIntros (_) "(V & d & T0)".
+    iExists (length vs * 2). iFrame.
+    iSplitR.
+    + iPureIntro. rewrite app_length. rew_qz. lia.
+    + iSplitR "T".
+      * iDestruct (diamonds_join with "[$]") as "?".
+        iApply (diamonds_eq with "[$]"). rewrite app_length /= //. rew_qz. lia.
+      * rewrite app_length. simpl length.
+        iApply (time_credit_weak with "T").
+        unfold time_reserve.
+        pose proof Nat.div_mod_eq (length vs) 2.
+        pose proof Nat.div_mul (length vs) 2.
+        do 2 destruct (decide _); lia.
 Qed.
 
-Lemma vector_set_amortized_spec `{!interpGS Σ} qz qp vs l i (x : val) :
-  qz ≠ 0%Qz ->
+Lemma vector_set_amortized_spec `{!interpGS Σ} vs l i (x : val) (q : Qp) :
   i < length vs ->
   CODE (vector_set [[#l, ^i, x]])
   SOUV {[l]}
-  PRE (vStackable x qp
-     ∗ x ↤?{qz} ∅
-     ∗ VectorAm qz qp vs l)
-  POST (fun r =>
-       vStackable (vs !!! i) qp
-     ∗ (vs !!! i) ↤?{qz} ∅
-     ∗ VectorAm qz qp (<[i:=x]> vs) l).
+  PRE (vStackable x q
+     ∗ x ↤?{q} ∅
+     ∗ VectorAm vs l)
+  POST (fun _ : () =>
+       (let '(v,q) := vs !!! i in vStackable v q ∗ v ↤?{q} ∅ )
+     ∗ VectorAm (<[i:=(x, q)]> vs) l).
 Proof.
-  iIntros (Hqz Hi) "(? & ? & V)".
-  iDestruct "V" as (cap) "(? & V)".
-  iPoseProof (vector_set_spec qz qp vs l cap i x with "[$]") as "A"; auto.
-  iApply (wps_mono with "A").
-  iIntros (?) "($ & $ & V)".
-  iExists cap; iFrame.
-  rewrite insert_length //.
-Qed.
-
-Lemma vector_get_amortized_spec `{!interpGS Σ} qz qp vs l i :
-  i < length vs ->
-  CODE (vector_get [[#l, ^i]])
-  SOUV {[l]}
-  PRE (VectorAm qz qp vs l)
-  POST (fun r => ⌜r = vs !!! i⌝ ∗ VectorAm qz qp vs l).
-Proof.
-  iIntros (Hi) "V".
-  iDestruct "V" as (cap) "(? & V)".
-  iPoseProof (vector_get_spec qz qp vs l cap i with "[$]") as "A"; auto.
+  iIntros (Hi) "(? & ? & V)".
+  iDestruct "V" as (cap) "(%Hcap & ? & ? & V)".
+  iPoseProof (vector_set_spec vs l cap i x with "[$]") as "A"; auto.
   iApply (wps_mono with "A").
   iIntros (?) "($ & V)".
   iExists cap; iFrame.
+  rewrite insert_length.
+  iSplitR; auto; iFrame.
 Qed.
 
-Lemma vector_pop_amortized_spec `{!interpGS Σ} qz qp vs l (x : val) :
-  qz ≠ 0%Qz ->
+Lemma vector_get_amortized_spec `{!interpGS Σ} vs l i :
+  i < length vs ->
+  CODE (vector_get [[#l, ^i]])
+  SOUV {[l]}
+  PRE (VectorAm vs l)
+  POST (fun r => ⌜r = (vs !!! i).1⌝ ∗ VectorAm vs l).
+Proof.
+  iIntros (Hi) "V".
+  iDestruct "V" as (cap) "(%Hcap & ? & ? & V)".
+  iPoseProof (vector_get_spec vs l cap i with "[$]") as "A"; auto.
+  iApply (wps_mono with "A").
+  iIntros (?) "($ & V)".
+  iExists cap; iFrame.
+  auto.
+Qed.
+
+Lemma vector_pop_amortized_spec `{!interpGS Σ} vs l (x : val) (q : Qp) :
   CODE (vector_pop [[#l]])
   SOUV {[l]}
-  PRE (VectorAm qz qp (vs ++ [x]) l)
+  PRE (VectorAm (vs ++ [(x, q)]) l ∗ $4)
   POST (fun r => ⌜r = x⌝
-      ∗ vStackable x qp
-      ∗ x ↤?{qz} ∅
-      ∗ VectorAm qz qp vs l).
+      ∗ vStackable x q
+      ∗ x ↤?{q} ∅
+      ∗ VectorAm vs l
+      ∗ ♢6).
 Proof.
-  iIntros (Hqz) "V".
-  iDestruct "V" as (cap) "(? & V)".
-  iPoseProof (vector_pop_spec qz qp vs l cap with "[$]") as "A"; auto.
-  iApply (wps_mono with "A").
-  iIntros (?) "($ & $ & $ & V)".
-  iExists cap; iFrame.
-  iApply (diamonds_le with "[$]"). rewrite app_length. lia.
+  iIntros "(V & T)".
+  iDestruct "V" as (cap) "(%Ucap & dn & dT & V)".
+  destruct (le_lt_dec (4 * length vs) cap) as [L|L].
+  - rewrite app_length in Ucap |- *; rew_qz.
+    simpl length in *.
+    mine (1 `max` (length vs * 2)) as "dia".
+    iDestruct (time_credit_join with "[$]") as "T".
+    iDestruct (time_credit_split_alt (S (1 `max` (length vs * 2)) + (length vs + 0)) with "[$]") as "(T1 & T)".
+    { revert L Ucap. remember (length vs) as s. clear Heqs. intros.
+      unfold time_reserve.
+      pose proof Nat.div_mod_eq cap 2.
+      pose proof Nat.mod_upper_bound cap 2.
+      destruct (decide _); lia. }
+    iPoseProof (vector_pop_spec_resize vs l cap with "[$]") as "A"; auto.
+    iApply (wps_mono with "A").
+    iIntros (?) "($ & $ & $ & V & dc & T0)".
+    iDestruct (diamonds_join with "[$]") as "?".
+    mine 6 as "dia".
+    iFrame "dia".
+    iExists _; iFrame.
+    iSplitR.
+    + iPureIntro. lia.
+    + iSplitR "T".
+      * iApply (diamonds_eq with "[$]"). rew_qz. lia.
+      * iApply (time_credit_weak with "T").
+        unfold time_reserve.
+        revert L Ucap. remember (length vs) as s. clear Heqs. intros.
+        pose proof Nat.div_mul s 2.
+        assert (s = 0 \/ s > 0) as [-> | Ps] by lia. by apply le_0_n.
+        replace (1 `max` (s * 2)) with (s * 2) by lia.
+        do 2 destruct (decide _); lia.
+
+  - rewrite app_length.
+    iPoseProof (vector_pop_spec_no_resize vs l cap with "[$]") as "A"; auto.
+    iApply (wps_mono with "A").
+    iIntros (?) "($ & $ & $ & V & T)".
+    mine 6 as "dia".
+    2: rewrite app_length in Ucap; rew_qz; lia.
+    iFrame "dia".
+    iExists cap; iFrame.
+    iDestruct (time_credit_join with "[$]") as "T".
+    iSplitR.
+    + iPureIntro. lia.
+    + iSplitR "T".
+      * iApply (diamonds_eq with "[$]"). rew_qz. lia.
+      * rewrite app_length in Ucap. simpl length in Ucap.
+        iApply (time_credit_weak with "T"). simpl length.
+        unfold time_reserve.
+        do 2 destruct (decide _); lia.
 Qed.
 
-Lemma vector_free_amortized  `{!interpGS Σ} qz qp vs l :
-  Stackable l 1%Qp ∗ l ↤ ∅ ∗ VectorAm qz qp vs l =#=∗
-  ♢(3 + length vs) ∗ †l
-    ∗ ([∗ list] v ∈ vs, v ↤?{qz} ∅)
-    ∗ ([∗ list] v ∈ vs, vStackable v qp).
+Lemma vector_pop_amortized_spec_lookup `{!interpGS Σ} (vs : list (val * Qp)) l :
+  vs ≠ [] ->
+  CODE (vector_pop [[#l]])
+  SOUV {[l]}
+  PRE (VectorAm vs l ∗ $4)
+  POST (fun r =>
+      let '(x, q) := vs !!! (length vs - 1) in
+        ⌜r = x⌝
+      ∗ vStackable x q
+      ∗ x ↤?{q} ∅
+      ∗ VectorAm (rev (tail (rev vs))) l
+      ∗ ♢6).
+Proof.
+  intros Hvs.
+  rewrite -(rev_involutive vs) in Hvs |- *.
+  destruct (rev vs) as [ | (x, q) ? ]. tauto.
+  iIntros "V".
+  rewrite /= list_lookup_total_middle ?app_length ?Nat.add_sub //.
+  iApply vector_pop_amortized_spec.
+  iExactEq = "V". iPureIntro. do 3 f_equal.
+  rewrite rev_app_distr /= rev_involutive //.
+Qed.
+
+Lemma vector_free_amortized  `{!interpGS Σ} vs l :
+  Stackable l 1%Qp ∗ l ↤ ∅ ∗ VectorAm vs l =#=∗
+  ♢(4 + 6 * length vs) ∗ †l
+  ∗ ([∗ list] vq ∈ vs, let '(v,q) := vq in vStackable v q ∗ v ↤?{q} ∅).
 Proof.
   iIntros "(Sl & Pl & V)".
   iIntros (? ? σ) "Hi".
-  iDestruct "V" as (cap) "(? & V)".
-  iPoseProof (vector_free  qz qp vs l cap
+  iDestruct "V" as (cap) "(%Ucap & dia & T & V)".
+  iPoseProof (vector_free  vs l cap
                with "[$Sl $Pl $V] Hi")
-    as ">(Hi & Sk & ? & ? & ?)".
+    as ">(Hi & Sk & ? & ?)".
   iFrame.
-  gather_diamonds. iModIntro.
-  iApply (diamonds_le with "[$]").
+  iDestruct (diamonds_join with "[$]") as "dia".
+  iModIntro.
+  iApply (diamonds_eq with "[$]").
+  rew_qz.
   lia.
+Qed.
+
+Tactic Notation "cleanup" :=
+  simpl;
+  repeat (
+      match goal with |- envs_entails _ (_ -∗ _) => iIntros "?" end
+     || match goal with |- envs_entails _ (∀ _, _) => iIntros (?) end
+     || match goal with |- envs_entails _ (♢ ?n ∗ _)%I => mine n as "_H"; [ iFrame "_H" | ..] end
+     || match goal with |- envs_entails _ ((♢ ?n ∗ _) ∗ _)%I => mine n as "_H"; [ iFrame "_H" | ..] end
+     || match goal with |- envs_entails _ ($ ?n ∗ _)%I => iDestruct (time_credit_split_alt n with "[$]") as "($ & ?)"; [ try lia | ]  end
+     || iDestruct (diamonds_join with "[$]") as "?"
+     || iDestruct select (_ ∗ _)%I as "(? & ?)"
+     || iDestruct select (⌜_⌝)%I as "%").
+
+Example amortized_example `{!interpGS Σ} :
+  CODE (
+      let: "v" := vector_create [[]] in
+      vector_push [["v", ^1]];;
+      vector_push [["v", ^2]];;
+      vector_push [["v", ^3]];;
+      vector_push [["v", ^4]];;
+      vector_push [["v", ^5]];;
+      vector_push [["v", ^6]];;
+      vector_push [["v", ^7]];;
+      vector_set [["v", ^0, ^11]];;
+      vector_set [["v", ^1, ^12]];;
+      vector_set [["v", ^1, ^22]];;
+      vector_pop [["v"]];;
+      vector_pop [["v"]];;
+      vector_pop [["v"]];;
+      vector_pop [["v"]];;
+      vector_pop [["v"]];;
+      let: "x" := vector_pop [["v"]] in
+      "x"
+    )
+  PRE (♢46 ∗ time_credit 73)
+  POST (fun res : val => ⌜res = 22⌝ ∗ ♢46).
+Proof.
+  iIntros "?".
+  wps_bind. wps_apply vector_create_amortized_spec. cleanup.
+  wps_bind. wps_apply vector_push_amortized_spec; auto. cleanup.
+  wps_bind. wps_apply vector_push_amortized_spec; auto. cleanup.
+  wps_bind. wps_apply vector_push_amortized_spec; auto. cleanup.
+  wps_bind. wps_apply vector_push_amortized_spec; auto. cleanup.
+  wps_bind. wps_apply vector_push_amortized_spec; auto. cleanup.
+  wps_bind. wps_apply vector_push_amortized_spec; auto. cleanup.
+  wps_bind. wps_apply vector_push_amortized_spec; auto. cleanup.
+  wps_bind. wps_apply vector_set_amortized_spec. simpl; lia. cleanup.
+  wps_bind. wps_apply vector_set_amortized_spec. simpl; lia. cleanup.
+  wps_bind. wps_apply vector_set_amortized_spec. simpl; lia. cleanup.
+  wps_bind. wps_apply vector_pop_amortized_spec_lookup. auto. cleanup.
+  wps_bind. wps_apply vector_pop_amortized_spec_lookup. auto. cleanup.
+  wps_bind. wps_apply vector_pop_amortized_spec_lookup. auto. cleanup.
+  wps_bind. wps_apply vector_pop_amortized_spec_lookup. auto. cleanup.
+  wps_bind. wps_apply vector_pop_amortized_spec_lookup. auto. cleanup.
+  wps_bind.
+  iApply wps_context_singleton; iFrame.
+  wps_apply vector_pop_amortized_spec_lookup. auto. cleanup.
+  iApply (wps_esupd _ _ _ _ (vector_free_amortized _ v)). iFrame. cleanup.
+  wps_val. iSplit. auto. rew_qz. iFrame.
+Unshelve.
+  all: try exact 1%Qp.
+  subst. auto.
 Qed.
