src/examples/dfs.v
@@ -1,0 +1,1006 @@
+From stdpp Require Import decidable binders gmultiset.
+From iris.proofmode Require Import proofmode environments.
+
+From iris.algebra Require Import gmap.
+
+From spacelambda.language Require Import notation.
+
+From spacelambda Require Import more_space_lang wp_all wp_spec triple closure.
+
+From spacelambda.examples Require Export tactics utils diaframe list.list list.iter_clo.
+From spacelambda.examples Require Export vector.
+
+Import language.
+Import notation.
+Import ListsOf.
+
+Context `{!interpGS Σ}.
+
+Definition VectorOf {A} (R : A -> val -> iProp Σ) (xs : list (A * Qp)) (l : loc) : iProp Σ :=
+  ∃ (vs : list (val * Qp)),
+    VectorAm vs l
+  ∗ ([∗ list] x; v ∈ xs; vs, R x.1 v.1 ∗ ⌜x.2 = v.2⌝ ∗ v.1 ↤? ∅ ∗ vStackable v.1 1%Qp)%I.
+
+Record graph := {
+  neighbors_at : list (list nat);
+  wf_neighbors_at : forall i l, l ∈ neighbors_at -> i ∈ l -> i < length neighbors_at
+}.
+
+Global Instance graph_size : Size graph := λ g, length (neighbors_at g).
+
+Definition has_edge (G : graph) i j := j ∈ neighbors_at G !!! i.
+
+Definition add_11 (l : list nat) := (λ n, (n, (1%Qz, 1%Qp))) <$> l.
+Definition add_1 (l : list (list nat)) := (λ l, (add_11 l, 1%Qp)) <$> l.
+
+Definition isGraph (G : graph) (g : loc) : iProp Σ :=
+  VectorOf
+    (fun L v => ∃ l, ⌜v=(#l)%V⌝ ∗ ListOf (fun (n : nat) v => ⌜v = (^n)%V⌝) L l)%I
+    (add_1 (neighbors_at G))
+    g.
+
+Definition number_of_edges (G : graph) := sum_list_with length (neighbors_at G).
+
+Inductive reachable (G : graph) : nat -> nat -> Prop :=
+  | reachable_self a : a < size G -> reachable G a a
+  | reachable_edge a b c : reachable G a b -> has_edge G b c -> reachable G a c.
+
+Lemma reachable_ind_unary (G : graph) (P : nat -> Prop) (src : nat) :
+  (forall i j, has_edge G i j -> P i -> P j) ->
+  (forall i j, reachable G i j -> P i -> P j).
+Proof.
+  intros H i j ij.
+  induction ij; firstorder.
+Qed.
+
+Lemma edge_bound_nodes G i j : has_edge G i j -> i < size G /\ j < size G.
+Proof.
+  destruct G as [l wf].
+  rewrite /has_edge /= /size /graph_size /= //.
+  change (j ∈ l !!! i → i < length l ∧ j < length l).
+  rewrite list_lookup_total_alt.
+  destruct (l !! i) eqn:Eli; rewrite /=.
+  - intros Hg; split.
+    + apply lookup_lt_is_Some_1; auto.
+    + pose proof (elem_of_list_lookup_2 _ _ _ Eli).
+      eapply wf; eauto.
+  - inversion 1.
+Qed.
+
+Lemma edge_inbound_node G i j : has_edge G i j -> i < size G.
+Proof.
+  apply edge_bound_nodes.
+Qed.
+
+Lemma edge_outbound_node G i j : has_edge G i j -> j < size G.
+Proof.
+  apply edge_bound_nodes.
+Qed.
+
+Definition count `{EqDecision A} (x : A) (l : list A) : nat := length (filter (eq x) l).
+
+Section count_facts.
+
+Context `{EqDecision A}.
+Context `{Inhabited A}.
+
+Lemma count_some (x : A) (l : list A) (i : nat) :
+  i < length l ->
+  l !!! i = x ->
+  1 ≤ count x l.
+Proof.
+  rewrite /count.
+  revert i; induction l as [ | b l ]; intros i Hi L. inversion Hi.
+  destruct i as [ | i ].
+  - simpl in *. subst.
+    rewrite filter_cons_True /= //; lia.
+  - simpl in *.
+    rewrite !filter_cons.
+    destruct (decide _) as [-> | n]; simpl; erewrite IHl; eauto; lia.
+Qed.
+
+Lemma count_remove (x y : A) (l : list A) (i : nat) :
+  x ≠ y ->
+  i < length l ->
+  l !!! i = x ->
+  count x l = count x (<[i:=y]> l) + 1.
+Proof.
+  rewrite /count.
+  revert i; induction l as [ | b l ]; intros i xy Hi L. inversion Hi.
+  destruct i as [ | i ].
+  - simpl in *. subst.
+    rewrite filter_cons_True /= // filter_cons_False /= //; lia.
+  - simpl in *.
+    rewrite !filter_cons.
+    destruct (decide _) as [-> | n]; simpl; erewrite IHl; eauto; lia.
+Qed.
+
+Lemma count_replicate (x : A) n : count x (replicate n x) = n.
+Proof.
+  unfold count.
+  induction n. easy.
+  rewrite /= filter_cons_True // /=.
+  congruence.
+Qed.
+
+Lemma count_true_false l : count true l + count false l = length l.
+Proof.
+  unfold count.
+  induction l as [ | [ | ] l ]; auto; rewrite !filter_cons; simpl; lia.
+Qed.
+
+End count_facts.
+
+(* [neighbors] is the list of neighbors remaining to be processed *)
+
+Record inv (G : graph) (src : nat) (marked : list bool) (stack neighbors : list nat) (measure : nat) := {
+  inv_length_marked : length marked = size G;
+  inv_source_node : src < size G;
+  inv_source : marked !!! src = true;
+  inv_stack : forall i, i ∈ stack -> i < size G /\ marked !!! i = true;
+  inv_true_reachable : forall i, i < size G -> marked !!! i = true -> reachable G src i;
+  inv_true_edges : forall i j, marked !!! i = true -> has_edge G i j -> i ∈ stack \/ marked !!! j = true \/ j ∈ neighbors;
+  inv_measure : measure = count false marked + length stack;
+  inv_stack_nodup : NoDup stack; (* required for length stack <= size G (< size G requires a little more) *)
+}.
+
+Lemma inv_stack_bound G a marked stack neigh measure :
+  inv G a marked stack neigh measure ->
+  length stack <= size G.
+Proof.
+  intros H.
+  destruct H.
+  rewrite -size_list_to_set //.
+  transitivity (length (seq 0 (size G))). 2: now rewrite seq_length.
+  rewrite -size_list_to_set. 2: apply NoDup_seq.
+  apply subseteq_size.
+  intros i.
+  rewrite !elem_of_list_to_set =>Hi.
+  destruct (inv_stack0 i Hi).
+  rewrite elem_of_seq.
+  lia.
+Qed.
+
+Tactic Notation "assert_specialize" hyp(H) :=
+  match type of H with
+    forall _ : ?a, _ =>
+    let Ha := fresh in
+    assert (Ha : a); [ | specialize (H Ha); clear Ha ]
+  end.
+
+Lemma initial_measure n a : a < n -> count false (<[a:=true]> (replicate n false)) = n - 1.
+Proof.
+  intros Ha.
+  pose proof count_replicate false n.
+  pose proof count_remove false true (replicate n false) a as R.
+  assert_specialize R. easy.
+  assert_specialize R. now rewrite replicate_length.
+  assert_specialize R. now rewrite lookup_total_replicate_2.
+  lia.
+Qed.
+
+Lemma inv_init G a : a < size G -> inv G a (<[a:=true]> (replicate (size G) false)) [a] [[]]%T (size G).
+Proof.
+  assert (Htrue : forall i, i < size G -> <[a:=true]> (replicate (size G) false) !!! i = true -> i = a). {
+    intros i Hi.
+    destruct (decide (a = i)) as [-> | n].
+    + rewrite list_lookup_total_insert // replicate_length. lia.
+    + rewrite list_lookup_total_insert_ne // lookup_total_replicate_2; lia.
+  }
+
+  split.
+  - rewrite insert_length replicate_length //.
+  - auto.
+  - apply list_lookup_total_insert.
+    rewrite replicate_length; lia.
+  - intros i. rewrite elem_of_list_singleton =>->.
+    rewrite list_lookup_total_insert // replicate_length; lia.
+  - intros i Hi Ci. apply Htrue in Ci; auto. subst. constructor. auto.
+  - intros i Hi Ci ij. apply Htrue in Ci. 2: now eapply edge_inbound_node; eauto.
+    left. apply elem_of_list_singleton, Ci.
+  - rewrite initial_measure /= //. lia.
+  - apply NoDup_singleton.
+Qed.
+
+Lemma inv_push_and_mark G a marked stack E i j measure :
+  marked !!! i = true ->
+  has_edge G i j ->
+  inv G a marked stack (j :: E) measure ->
+  marked !!! j = false ->
+  inv G a (<[j:=true]> marked) (stack ++ [j]) E measure.
+Proof.
+  intros Ci ij [] H0.
+  assert (i < size G) as Ni by now eapply edge_inbound_node; eauto.
+  assert (j < size G) as Nj by now eapply edge_outbound_node; eauto.
+  assert (j < length marked) by now rewrite -inv_length_marked0 in Nj.
+  split; auto.
+  - rewrite insert_length //.
+  - destruct (decide (a = j)) as [->|aj].
+    + rewrite list_lookup_total_insert //.
+    + rewrite list_lookup_total_insert_ne //.
+  - intros k. rewrite elem_of_app. intros [Hk | jk].
+    + destruct (inv_stack0 k); auto. split; auto.
+      destruct (decide (k = j)) as [->|kj].
+      * rewrite list_lookup_total_insert //.
+      * rewrite list_lookup_total_insert_ne //.
+    + apply elem_of_list_singleton in jk; subst. split.
+      * eapply edge_outbound_node; eauto.
+      * rewrite list_lookup_total_insert //.
+  - intros k Hk.
+    destruct (decide (k = j)) as [->|kj].
+    * rewrite list_lookup_total_insert //. intros _.
+      apply reachable_edge with i; auto.
+    * rewrite list_lookup_total_insert_ne //.
+      apply inv_true_reachable0; auto.
+  - intros ii k.
+    destruct (decide (ii = j)) as [->|iij].
+    + intros _ _. left. apply elem_of_app. right. left.
+    + rewrite list_lookup_total_insert_ne //.
+      intros Hi ik.
+      specialize (inv_true_edges0 ii k Hi ik).
+      destruct inv_true_edges0 as [HE | [HE | HE] ].
+      * left. apply elem_of_app. left; auto.
+      * right. left. destruct (decide (j = k)) as [->|jk].
+        -- rewrite list_lookup_total_insert //.
+        -- rewrite list_lookup_total_insert_ne //.
+      * inversion HE; subst.
+        -- rewrite list_lookup_total_insert //. auto.
+        -- auto.
+  - rewrite inv_measure0 (count_remove _ true _ j) // app_length /=. lia.
+  - rewrite -Permutation_cons_append. constructor; auto.
+    intros Hj. destruct (inv_stack0 j Hj). congruence.
+Qed.
+
+Definition array_fill : val :=
+  μ: "self", [["dst", "v", "i", "n"]],
+    let: "neq" := "n" '- "i" in
+    if: "neq" then
+      "dst".["i"] <- "v";;
+      let: "i" := "i" '+ ^1 in
+      "self" [["dst", "v", "i", "n"]]
+    else
+      ()%V.
+
+Lemma array_fill_spec_from_unit_to_nat `{!interpGS Σ} (dst : loc) (v i n : nat) :
+  CODE (array_fill [[#dst, ^v, ^i, ^(i + n)]])
+  SOUV {[dst]}
+  PRE (dst ↦ BBlock (replicate i (^v)%V ++ replicate n ()%V))
+  POST (fun _ : unit => dst ↦ BBlock (replicate (i + n) (^v)%V)).
+Proof.
+  iIntros "Hdst".
+  iInduction n as [ | len ] "IH" forall (i).
+  - wps_call.
+    wps_bind. wps_val.
+    wps_if. rewrite decide_False. 2:lia.
+    wps_val. rewrite Nat.add_0_r. done.
+  - wps_call.
+    wps_bind. wps_val.
+    wps_if. rewrite decide_True. 2:lia.
+    wps_bind. wps_store.
+    replace (<[i:=^v]> (replicate i ^v ++ () :: replicate len ()))%V
+      with  (replicate (i + 1) ^v ++ replicate len ())%V
+      by rewrite insert_app_r_alt ?replicate_length ?Nat.sub_diag /= //
+           replicate_plus -app_assoc /= //.
+    wps_bind. wps_val.
+    fold array_fill.
+    change (enc (i + 1)) with (^(i + 1))%V.
+    replace (^(i + S len))%V with (^(i + 1 + len))%V by (f_equal; lia).
+    iSpecialize ("IH" $! (i + 1) with "[$]").
+    iApply (wps_mono with "[IH]").
+    iApply "IH".
+    replace (i + 1 + len)%nat with (i + S len)%nat by lia.
+    auto.
+Unshelve.
+  now constructor.
+  now rewrite app_length replicate_length /=; lia.
+Qed.
+
+Definition reachable_imperative : val :=
+  (* let reachable_imperative g a b = *)
+  λ: [["g", "a", "b"]],
+    (* let n = Graph.nb_nodes g in *)
+    let: "n" := vector_size [["g"]] in
+    (* let c = Array.make n false in *)
+    let: "c" := alloc "n" in
+    array_fill [["c", 0, 0, "n"]];;
+    (* let s = Stack.create() in *)
+    let: "s" := vector_create [[]] in
+    (* c.(a) <- true; *)
+    "c".["a"] <- ^1;;
+    (* Stack.push a s; *)
+    vector_push [["s", "a"]];;
+    (* while not (Stack.is_empty s) do *)
+    (μ: "while", [["s", "c", "g"]],
+        let: "not_empty" := vector_size [["s"]] in
+        if: "not_empty" then
+          (* let i = Stack.pop s in *)
+          let: "i" := vector_pop [["s"]] in
+          (* let f j = *)
+          let: "f" := mk_clo BAnon ["j":binder] (
+            (* if not c.(j) then begin *)
+            let: "marked" := "c".["j"] in
+            if: "marked" then ()%V else (
+                (* c.(j) <- true; *)
+                "c".["j"] <- 1;;
+                (* Stack.push j s; *)
+                vector_push [["s", "j"]]
+              (* end); *)
+              )
+          (* in *)
+          ) in
+          (* Graph.iter_edges g i f *)
+          let: "edges" := vector_get [["g", "i"]] in
+          list_iter [["f", "edges"]];;
+          (* done; *)
+          "while" [["s", "c", "g"]]
+        else ()%V) [["s", "c", "g"]];;
+    (* c.(b) *)
+    "c".["b"].
+
+(** Change [wps X t Q] into two goals [wps X t R] and [∀v, Q v -∗ R v] *)
+Ltac wps_conseq_post R :=
+  match goal with
+  | |- envs_entails ?Δ (wps ?X ?t ?Q) =>
+      let H := fresh "Hwps_conseq_post" in
+      assert (envs_entails Δ (wps X t R)) as H;
+      [ | iApply (wps_mono with "[-]"); [ apply H | clear H ] ]
+  end.
+
+Tactic Notation "iAssertSpecialize" constr(iris_hyp) :=
+  match goal with
+  | |- context[Esnoc _ (INamed iris_hyp) (?B -∗ _)%I] =>
+      iAssert B as "_tmp";
+      [ | iSpecialize (iris_hyp with "_tmp"); iClear "_tmp" ]
+  | |- context[Esnoc _ (INamed iris_hyp) (bi_impl ?B _)%I] =>
+      (* bi_impl is the -> implication, it should not be useful with a "with" clause *)
+      iAssert B as "_tmp";
+      [ | iSpecialize (iris_hyp with "_tmp"); iClear "_tmp" ]
+  end.
+
+Tactic Notation "iAssertSpecialize" constr(iris_hyp) "with" constr(iris_hyps_for_the_assert) :=
+  match goal with
+  | |- context[Esnoc _ (INamed iris_hyp) (?B -∗ _)%I] =>
+      iAssert B with iris_hyps_for_the_assert as "_tmp";
+      [ | iSpecialize (iris_hyp with "_tmp") ]
+  end.
+
+Definition HIDDEN {A : Type} {x : A} := x.
+
+Tactic Notation "iHide" constr(iris_hyp) :=
+  match goal with
+  | |- context[Esnoc ?G (INamed iris_hyp) ?H] =>
+      change (Esnoc G (INamed iris_hyp) H)
+      with   (Esnoc G (INamed iris_hyp) (@HIDDEN _ H))
+  end.
+
+Tactic Notation "iShow" constr(iris_hyp) :=
+  match goal with
+  | |- context[Esnoc ?G (INamed iris_hyp) (@HIDDEN _ ?H)] =>
+      change (Esnoc G (INamed iris_hyp) (@HIDDEN _ H))
+      with   (Esnoc G (INamed iris_hyp) H)
+  end.
+
+Ltac cleanup_Stackable :=
+  repeat
+    match goal with
+    | |- context[@own _ ?A _ _ (auth.auth_frag {[?l := ?q]})] =>
+        change (@own _  A _ _ (auth.auth_frag {[ l :=  q]}))%I
+        with (Stackable l q)
+    end.
+
+Tactic Notation "wps_weak" uconstr(r1) :=
+  match goal with
+  | |- envs_entails _ (wps (Some ?r2) ?t ?Q) =>
+      iAssert (wps (Some r1) t Q) with "[-]" as "_tmp";
+      [ | iApply (wps_weak with "_tmp") ];
+      swap 1 2
+  end.
+
+Tactic Notation "wps_weak" uconstr(r1) "by" tactic(t) :=
+  wps_weak r1; [ by t | ].
+
+Definition State (G : graph) (g lmarked lstack : loc) (source : nat) (marked : list bool) (stack : list nat) (neighbors : list nat) (meas : nat) : iProp Σ :=
+    lmarked ↦ BBlock (val_nat <$> (Nat.b2n <$> marked))
+  ∗ ♢((size G - length stack) * 6)%nat
+  ∗ $(count false marked * 11 + length stack * 4)
+  ∗ VectorAm ((fun n => ((^n)%V, 1%Qp)) <$> stack) lstack
+  ∗ ⌜inv G source marked stack neighbors meas⌝.
+
+Lemma inv_end G a C meas :
+  inv G a C [] [] meas ->
+  forall b, b < size G -> C !!! b = true ∧ reachable G a b ∨ C !!! b = false ∧ ¬ reachable G a b.
+Proof.
+  intros [_ _ Ca _ Hreach Hedges].
+  cut ( ∀ b : nat, reachable G a b -> b < size G → C !!! b = true). {
+    intros H b Hb. destruct (C !!! b) eqn:Cb.
+    - left. now specialize (Hreach b Hb Cb).
+    - right. split; auto. intros Rb. specialize (H b Rb Hb). congruence.
+  }
+  intros b ab Hb.
+  refine (reachable_ind_unary G (λ b, C !!! b = true) 42 _ a b ab Ca).
+  intros i j ij Ci.
+  destruct (Hedges i j Ci ij) as [F | [? | F] ]; auto; inversion F.
+Qed.
+
+Lemma inv_marked G src marked stack E i j meas :
+  has_edge G i j ->
+  marked !!! j = true ->
+  inv G src marked stack (j :: E) meas ->
+  inv G src marked stack E meas.
+Proof.
+  intros ij Cj []; constructor; auto.
+  intros a b Ca ab.
+  destruct (inv_true_edges0 a b Ca ab) as [ ? | [ ? | jE ] ]; auto.
+  inversion jE; subst; intuition.
+Qed.
+
+Lemma neighbors_char G i j l : neighbors_at G !! i = Some l -> has_edge G i j <-> j ∈ l.
+Proof.
+  intros Hl.
+  unfold has_edge.
+  erewrite list_lookup_total_correct; eauto.
+Qed.
+
+Lemma neighbors_char_add_1 G i j l q : add_1 (neighbors_at G) !! i = Some (l, q) -> has_edge G i j <-> j ∈ l.*1.
+Proof.
+  intros Hl.
+  rewrite neighbors_char; eauto.
+  unfold add_1 in Hl.
+  apply list_lookup_fmap_inv in Hl.
+  destruct Hl as (l1 & [=->->] & ->).
+  f_equal.
+  induction l1; simpl; f_equal; auto.
+Qed.
+
+Lemma inv_stage_neighbors G a marked stack cur l meas :
+  neighbors_at G !! cur = Some l ->
+  inv G a marked (stack ++ [cur]) [] meas ->
+  inv G a marked stack l (meas - 1).
+Proof.
+  intros Hl [].
+  constructor; auto.
+  - intros. apply inv_stack0. rewrite elem_of_app. auto.
+  - intros i j Hi ij.
+    destruct (inv_true_edges0 i j Hi ij) as [Hj | [ Hj | Hj ] ].
+    + rewrite elem_of_app elem_of_list_singleton in Hj. destruct Hj as [Hj | ->]. now auto.
+      right. right.
+      eapply neighbors_char; eauto.
+    + auto.
+    + inversion Hj.
+  - rewrite app_length /= in inv_measure0. lia.
+  - eapply (NoDup_app stack [cur]); auto.
+Qed.
+
+Lemma Qp_Qz_1 : (1%Qp : Qz) = 1%Qz.
+Proof.
+  rewrite -pos_to_qz_through_nat.
+  apply Qz_to_Qc_inj_iff.
+  rewrite nat_to_Qz_to_Qc //.
+Qed.
+
+(** Explanation of space complexity:
+ - 4: creating stack
+ - size G * 6: six times the maximum size of the stack (could be refined to size G - 1)
+ - size G: boolean array for marking as marked
+ - 3: allocating the closure passed to list_iter
+ - 3: list_iter's internal closure
+*)
+
+(** Explanation of time complexity:
+ - 7 * size G: pushing all nodes on the stack
+ - 4 * size G: popping all nodes
+
+Note that we should also have O(number_of_edges G) because we iterate on all
+neighbors every time, but time complexity is not accounted for in list_iter, and
+this project is not about time complexity, so we only mention time complexity
+here because we did for the amortized analysis for vectors (for which it was
+useful to check that our implementation for amortized space complexity was not
+at the expense of time complexity). *)
+
+Lemma reachable_imperative_spec g G (a b : nat) qg :
+  a < size G ->
+  b < size G ->
+  CODE (reachable_imperative [[g, a, b]])
+  PRE (isGraph G g ∗ Stackable g qg ∗ ♢(size G * 7 + 10) ∗ $(size G * 11))
+  POST (fun (r : nat) =>
+       isGraph G g ∗ Stackable g qg ∗ ♢(size G * 7 + 10)
+     ∗ ⌜r = 1 /\ reachable G a b \/ r = 0 /\ ~reachable G a b⌝).
+Proof.
+  iIntros (Ha Hb) "(G & Sg & D & T)".
+  iDestruct "G" as (locs) "(Vg & Hlocs)".
+  wps_call.
+
+  iAssert ⌜length locs = size G⌝%I as %Llocs.
+  { iPoseProof (big_sepL2_length with "[$]") as "<-"; rewrite map_length //. }
+
+  (** let n = vector_size g *)
+  wps_bind_nofree.
+  wps_apply vector_size_amortized_spec.
+  iDestruct select (⌜_⌝ ∗ _)%I as "(%En & Vg)".
+  rename v into n.
+
+  (** let marked = alloc n *)
+  wps_bind.
+  wps_alloc.
+  iIntros "Sg".
+  rename l into lmarked.
+  iDestruct select (_ ∗ _)%I as "(Pm & Sm)".
+
+  (** array_fill marked 0 0 n *)
+  wps_bind.
+  wps_apply array_fill_spec_from_unit_to_nat.
+  clear v.
+  iIntros "(Sm & Sg)".
+
+  (** let stack = vector_create () *)
+  wps_bind.
+  iDestruct (time_credit_split_alt 0 with "[$]") as "(T0 & T)". lia.
+  mine 4.
+  wps_apply vector_create_amortized_spec.
+  rename v into lstack.
+  iIntros "(Sm & Sg)".
+  iDestruct select (_ ∗ _ ∗ _)%I as "(Vstack & Ss & Ps)".
+
+  (** marked[a] <- 1 *)
+  wps_bind.
+  (* Fail wps_store. *)
+  do 7 iStepS.
+  iDestruct select (Stackables _) as "((Ss & Sm) & Sg)".
+  match goal with x : unit |- _ => clear x end.
+
+  (** stack.push(a) *)
+  wps_bind.
+  iDestruct (time_credit_split_alt 7 with "[$]") as "(T0 & T)". lia.
+  mine 6.
+  unshelve wps_apply vector_push_amortized_spec. exact 1%Qp.
+  match goal with x : unit |- _ => clear x end.
+  iIntros "((Ss & Sm) & Sg)".
+
+  set (μ: _, _, _) as outer_loop.
+
+  iRename select (♢ _)%I into "D6".
+  mine ((size G - 1) * 6) as "D".
+
+  iAssert (State G g lmarked lstack a (<[a:=true]> (replicate (length locs) false)) [a] [] (size G))%I
+    with "[-D6 Ss Sm Sg Pm Ps Vg Hlocs]"
+    as "Hinv".
+  {
+    iFrame.
+    iRename select (lmarked ↦ _)%I into "Hmarked".
+    iSplitL "Hmarked".
+    { iExactEq = "Hmarked". iPureIntro. do 2 f_equal.
+      now rewrite !list_fmap_insert !fmap_replicate //. }
+    iSplitL "T".
+    { iExactEq = "T". iPureIntro. do 2 f_equal.
+      pose proof count_remove false true (replicate (length locs) false) a as M.
+      assert_specialize M. easy.
+      assert_specialize M. rewrite replicate_length Llocs //.
+      assert_specialize M. rewrite lookup_total_replicate_2 // Llocs //.
+      rewrite Llocs count_replicate in M.
+      rewrite M Llocs /=.
+      lia. }
+    iPureIntro.
+    rewrite Llocs. apply inv_init; auto.
+  }
+
+  iDestruct "Sm" as "(Sm1 & Sm2)".
+  iDestruct "Ss" as "(Ss1 & Ss2)".
+  iDestruct "Sg" as "(Sg1 & Sg2)".
+  wps_bind.
+  wps_context lstack.
+  cleanup_Stackable.
+  wps_context g.
+  set (x := (_ - _)%nat); assert (x = 6)%nat as -> by lia.
+
+  (** outer loop: induction on the measure *)
+  generalize [a]; intros stack.
+  generalize (<[a:=true]> (replicate (length locs) false)); intros marked.
+  remember (size G) as meas eqn:Emeas.
+  (* assert (0 < meas) as Hm by lia. *)
+  rewrite Emeas in Llocs Ha Hb. rewrite {2}Emeas. clear Emeas.
+  (* induction on "meas+1" to avoid the base case, i.e. we show
+     ∀x(x>0⇒P(x-1))⇒P(x) instead of P(0)∧(∀x,P(x)⇒P(x+1)) *)
+  assert (exists m, meas + 1 = m) as (m, Hm) by eauto;
+  iInduction m as [ | m ] "IH" forall (meas Hm stack marked);
+    [ lia | assert (m = meas) as -> by lia; clear Hm ].
+
+  iDestruct "Hinv" as "(Hmarked & D & T & Vs & %Hinv)".
+  wps_call. fold outer_loop.
+
+  (** let not_empty = vector_size stack *)
+  wps_bind_nofree.
+  wps_apply vector_size_amortized_spec.
+  simpl.
+  rename v into nstack.
+  iDestruct select (_ ∗ _)%I as "(%Heq_nstack & Vs)".
+
+  (** if stack is empty, the outer loop ends *)
+  destruct (decide (stack = [])) as [-> | stack_not_empty].
+  {
+    iClear "IH".
+    wps_if.
+    wps_val.
+    iIntros "? ? ?".
+    iDestruct (Stackable_join g with "[$] [$]") as "Sg".
+    iDestruct (Stackable_join lstack with "[$] [$]") as "Ss".
+    iDestruct (Stackable_join lmarked with "[$] [$]") as "Sm".
+
+    (** freeing [lmarked] after load, as if there were a let *)
+    iApply wps_end.
+
+    wps_context lmarked.
+    rewrite !Qp_div_2.
+
+    (** freeing vector stack *)
+    iApply (wps_esupd (A := nat) _ _ _ _ (vector_free_amortized [] lstack)).
+    iFrame.
+    iIntros "(Ds & ds & true)".
+
+    (** computing return value *)
+    iStepS.
+    iExists _, _, _. iFrame.
+    iSplit.
+    { iPureIntro.
+      rewrite !fmap_length //.
+      destruct Hinv. lia. }
+    iSplit.
+    { iPureIntro.
+      destruct Hinv.
+      rewrite !list_lookup_total_fmap ?fmap_length; try lia.
+      reflexivity. }
+    iIntros "Hmarked Sm".
+
+    (** freeing [lmarked] *)
+    wps_free lmarked as "(Dm & dl')".
+    wps_val.
+
+    (** establishing spec's postcondition *)
+    iFrame "Sg".
+    iSplitL "Vg Hlocs". now iExists _; iFrame.
+    iSplitL "D6 D Ds Dm".
+    - do 3 iDestruct (diamonds_join with "[$]") as "ds".
+      iExactEq = "ds". iPureIntro. f_equal.
+      rew_qz.
+      rewrite !fmap_length.
+      destruct Hinv.
+      lia.
+    - iClear "T" (* here, throwing away $11 * number of unreachable nodes *).
+      iPureIntro.
+      eapply inv_end in Hinv; eauto.
+      destruct Hinv as [ [-> H] | [-> H] ]; [left | right]; split; auto.
+  }
+
+  (** otherwise the stack is not empty *)
+  wps_if.
+  rewrite decide_True.
+  2: now destruct stack; tauto || simpl in *; lia.
+
+  (* using wps_let_empty instead of wps_bind, which takes more than 30 minutes *)
+  (* Fail Timeout 500 wps_bind. *)
+  Time simplify_substs. (* TODO: 10 seconds *)
+  iApply wps_let_empty.
+  reflexivity.
+  {
+    rewrite /locs /location_tm /=.
+    apply union_least. 2:now set_solver.
+    etransitivity. now apply locs_subst.
+    apply union_least. now set_solver.
+    etransitivity. now apply locs_subst.
+    rewrite /syntax.locs /location_tm /=. rewrite locs_mk_clo.
+    set_solver.
+  }
+
+  (** let [current_node] be the node we pop out *)
+  destruct (@exists_last _ stack ltac:(auto)) as (stack' & current_node & ->).
+  rewrite fmap_app /=.
+  wps_apply vector_pop_amortized_spec.
+  iDestruct (time_credit_split_alt 4 with "[$]") as "($ & T)".
+  { rewrite app_length /=. lia. }
+  iIntros (v1) "(-> & _ & _ & Vstack & D')".
+
+  (** let f = our closure *)
+  Time simplify_substs. (* 2.5 seconds *)
+  wps_bind_nofree.
+
+  (* we choose the specification of the closure we are allocating *)
+
+  Definition push_and_mark_spec G g lmarked lstack a (_ : loc) (args : list val) (t : tm) (spec : iProp Σ) :=
+    (∀  (marked : list bool) (stack : list nat) (neighbors : list nat) (i j meas : nat),
+      ⌜args = [ ^j ]%V⌝ -∗
+      ⌜has_edge G i j /\ marked !!! i = true⌝ -∗
+      State G g lmarked lstack a marked stack (j :: neighbors) meas -∗
+      wps (Some {[g; lstack; lmarked]}) t
+      (λ _ : (),
+          State G g lmarked lstack a
+            (if (marked !!! j : bool) then marked else <[j := true]> marked)
+            (if (marked !!! j : bool) then stack else stack ++ [j])
+            neighbors meas
+          ∗ spec)
+    )%I.
+
+  assert (LNE (push_and_mark_spec G g lmarked lstack a)) by lne.
+  rewrite subst_subst_commut. 2: easy.
+
+  (* we apply wps_mk_spec, which will give us the hypothesis that f satisfies push_and_mark_spec G *)
+  wps_apply (wps_mk_spec (push_and_mark_spec G g lmarked lstack a)
+    [("c", #lmarked)%V; ("s", #lstack)%V]
+    [(1/2)%Qp : Qz; (1/2)%Qp : Qz] ).
+  1-4: now compute_done.
+
+  (** The body of the closure satisfies push_and_mark_spec *)
+  {
+    (* first some closure bookkeeping *)
+    iModIntro.
+    iIntros (l args len_args) "Spec".
+    destruct args as [ | arg [ | ? ? ] ]. 1,3: now inversion len_args.
+    simpl.
+    clear marked Hinv.
+    iIntros (marked stack E i j meas') "%Earg". inversion Earg. subst arg.
+    iIntros "(%Hij & %Ci) (Hmarked & D & T & Vstack & %Hinv)".
+    assert (j < length marked) as Hj. {
+      destruct Hinv.
+      rewrite inv_length_marked0.
+      eapply edge_outbound_node; eauto.
+    }
+    assert (j < length (Nat.b2n <$> marked)) as Hj' by rewrite map_length //.
+
+    (** if marked[j] *)
+    wps_bind.
+    wps_load.
+
+    rewrite !list_lookup_total_fmap //.
+    destruct (marked !!! j) eqn:Cj.
+    - (** if marked[j], nothing happens *)
+      wps_if.
+      wps_val.
+      iFrame.
+      iPureIntro.
+      eapply inv_marked; eauto.
+
+    - (** otherwise *)
+      wps_if.
+
+      (** marked[j] := true *)
+      wps_bind.
+      wps_store.
+
+      (** preparing invariant in advance so that we can extract space credits from invariant *)
+      assert (Hinv' : inv G a (<[j:=true]> marked) (stack ++ [j]) E meas')
+        by now apply inv_push_and_mark with i.
+      assert (Hlen : length stack < size G). {
+        apply inv_stack_bound in Hinv'.
+        rewrite app_length /= in Hinv'.
+        lia.
+      }
+
+      (** stack.push(j) *)
+      mine 6.
+      iDestruct (time_credit_split_alt 7 with "[$]") as "(T7 & T)".
+      { eapply (count_some _ _ j) in Cj; auto. lia. }
+      wps_apply vector_push_amortized_spec.
+      unfold State.
+      rewrite !list_fmap_insert !list_lookup_total_fmap //.
+      rewrite fmap_app.
+      iFrame.
+      iSplitL "D".
+      { iExactEq = "D".
+        iPureIntro. f_equal. rewrite app_length /=.
+        rew_qz; lia. }
+      iSplit; auto.
+      { iExactEq = "T". iPureIntro. f_equal.
+        rewrite app_length /= (count_remove false true marked j) //.
+        lia. }
+  }
+
+  (** finishing wps_mk_spec's bookkeeping *)
+  simpl.
+  mine 3.
+  iFrame.
+  rewrite /group_pointedbys Qp_to_Qz_mul_distr Qp_Qz_1.
+  change ((1 * / 2)%Qz) with ((1 / 2)%Qz).
+  rewrite -{4 5}(Qz_div_2 1).
+  rewrite /=.
+  iDestruct (mapsfrom_split_empty with "Ps") as "(Ps1 & $)".
+  iDestruct (mapsfrom_split_empty with "Pm") as "(Pm1 & $)".
+  iIntros (lclosure) "(Pc & Sc & Hclosure)".
+
+  (** let edges = neighbors of current_node *)
+  wps_bind.
+  iPoseProof (big_sepL2_length with "[$]") as "%lenadj".
+  assert (current_node < length locs) as li.
+  { rewrite -lenadj map_length.
+    destruct Hinv.
+    specialize (inv_stack0 current_node).
+    assert_specialize inv_stack0.
+    { apply elem_of_app. right. left. }
+    destruct inv_stack0 as [Hcur _].
+    apply Hcur.
+  }
+
+  Time wps_apply vector_get_amortized_spec. (* TODO 8 sec *) assumption.
+  iDestruct select (_ ∗ _)%I as "(-> & Vg)".
+  iIntros "Sc".
+
+  (** extracting the neighbors from the graph's vector (some bookkeeping is due
+  to the more general VectorOf instead of a custom version) *)
+  pose (R_isnat := λ n v, ⌜v = (^n)%V⌝%I : iProp Σ).
+  fold R_isnat.
+  pose proof lookup_lt_is_Some_2 _ _ li as ((v_ & qn) & Eneighbors).
+  set (ll := add_1 _); assert (current_node < length ll) as lli by now subst ll; congruence; subst ll.
+  pose proof lookup_lt_is_Some_2 _ _ lli as ((neighbors_qs, q_) & Hneighbors_qs).
+  iDestruct (big_sepL2_lookup_acc with "Hlocs") as "((Hneighbors & %Eq_ & Pn & Sn) & Hlocs_hole)"; eauto.
+  simpl in Eq_; subst q_.
+  iDestruct "Hneighbors" as (lneighbors) "(%Heq & Hneighbors)".
+  simpl in Heq; subst v_; simpl.
+
+  (** iteration on current_node's neighbors *)
+  wps_bind.
+  wps_context lclosure.
+  wps_context lneighbors.
+
+  pose (I := fun (remaining_neighbors : list nat) => (
+      Spec 1 [((#lmarked)%V, (1 / 2)%Qz); ((#lstack)%V, (1 / 2)%Qz)] (push_and_mark_spec G g lmarked lstack a) lclosure
+    ∗ ⌜Forall (has_edge G current_node) remaining_neighbors⌝
+    (* Stackables required because closure needs to be shown to not free g *)
+    ∗ Stackable g (qg / 2)%Qp
+    ∗ Stackable lstack (1 / 2)%Qp
+    ∗ Stackable lmarked (1 / 2)%Qp
+    ∗ ∃ stack marked,
+      ⌜marked !!! current_node = true⌝
+      ∗ State G g lmarked lstack a marked stack remaining_neighbors (meas - 1)
+    )%I : iProp Σ).
+
+  iPoseProof (iter_spec_remaining I R_isnat neighbors_qs lneighbors lclosure 1)
+    as "-#iter"; [ auto | ].
+  mine 2 as "D2".
+  erewrite list_lookup_total_correct; [ | eassumption ]; simpl.
+
+  iAssertSpecialize "iter" with "[-IH Pm1 Ps1 Vg Hlocs_hole Pn iter D']".
+
+  iSplit.
+  { (** each iteration of the closure preserves the invariant *)
+    iModIntro.
+    iIntros (neighbor v_ remaining_neighbors) "(I & Rxy)".
+    iDestruct "Rxy" as "->".
+    iDestruct "I" as "(Hclosure & %Hedges & Sg & Ss & Sm & Hstate)".
+    iApply (wpc_call_spec with "Hclosure").
+    now change ([(^neighbor)%V : tm]) with (tm_val <$> [(^neighbor)%V]); reflexivity.
+    reflexivity.
+    iIntros (body) "Hclosure".
+    iDestruct "Hstate" as (stack_ marked_) "Hstate".
+    iDestruct "Hstate" as "(%Hmarked_cur & Hmarked & D & T & Vstack & %Hinv_)".
+    iSpecialize ("Hclosure" $! marked_ stack_ remaining_neighbors current_node neighbor (meas - 1)).
+    iAssertSpecialize "Hclosure". easy.
+    iAssertSpecialize "Hclosure". now iPureIntro; split; auto; inversion Hedges; subst; auto.
+    iSpecialize ("Hclosure" with "[$Vstack $Hmarked $D $T]"); auto.
+    rewrite -(wps_eq _ _ (Some _)).
+    wps_context g.
+    wps_context lstack.
+    wps_context lmarked.
+    wps_weak {[g; lstack; lmarked]} by set_solver.
+    iApply (wps_mono with "Hclosure").
+    iIntros ([]) "(Hstate & Hclosure) Sm Ss Sg". iSplit. done.
+    iFrame.
+    iSplit. now inversion Hedges; subst; auto.
+    iExists _, _. iFrame.
+    iPureIntro.
+    destruct (marked_ !!! neighbor) eqn:E; auto.
+    destruct (decide (neighbor = current_node)) as [-> | n].
+    - rewrite list_lookup_total_insert //; congruence.
+    - rewrite list_lookup_total_insert_ne //.
+  }
+
+  { (** we establish the invariant before list iter *)
+    iFrame.
+    iSplit.
+    * (* the list only contains neighbors *)
+      iPureIntro.
+      apply Forall_forall; intros j Hj.
+      eapply neighbors_char_add_1; eauto.
+    * iExists stack', marked.
+      iFrame.
+      iSplit.
+      { iPureIntro.
+        inversion Hinv.
+        apply inv_stack0. rewrite elem_of_app elem_of_list_singleton.
+        auto. }
+      iSplitL "D6 D".
+      { iDestruct (diamonds_join with "[$]") as "D".
+        iExactEq = "D". iPureIntro. f_equal.
+        rewrite app_length /=.
+        rew_qz.
+        cut (length stack'< size G). lia.
+        apply inv_stack_bound in Hinv.
+        rewrite app_length /= in Hinv.
+        lia. }
+      iSplitL "T".
+      { iExactEq = "T". iPureIntro. do 2 f_equal.
+        rewrite app_length /=. lia. }
+      iPureIntro.
+      eapply inv_stage_neighbors; eauto.
+      unfold add_1 in *.
+      apply list_lookup_fmap_inv in Hneighbors_qs.
+      destruct Hneighbors_qs as (l1 & [=->->] & ->).
+      f_equal. induction l1; simpl; f_equal; auto.
+  }
+
+  (** the specification of "iter" has been specialized *)
+
+  wps_weak {[lneighbors; lclosure]} by set_solver.
+  (* list_iter returns unit, but wps_binds asks us to prove it for any val, so: *)
+  rewrite wps_return_unit_iff.
+  (* Fail wps_apply "iter". (* Tactic failure: iPoseProof: "iter" not found *) *)
+  iApply (wps_mono with "iter").
+
+  (** we get back list_iter's final invariant *)
+  iIntros (?) "(-> & D2 & Hneighbors & I & Pc) Sn Sc".
+  iDestruct "I" as "(Hspec & %Htrue & Sg & Ss & Sm & I)".
+  iDestruct "I" as (stack marked') "(%Hmarkedcur & Hmarked & D & T & Vs & %Hinv')".
+
+  (** we free the closure *)
+  iApply wps_esupd. set_solver. apply (spec_esupd_free lclosure).
+  iFrame.
+  iIntros "(D3 & Pm2 & Ps2 & _)". simpl.
+  iDestruct (mapsfrom_join lmarked with "[$] [$]") as "Pm".
+  iDestruct (mapsfrom_join lstack with "[$] [$]") as "Ps".
+  rewrite left_id. assert (1 / 2 + 1 / 2 = 1)%Qz as -> by now rewrite Qz_div_2.
+
+  (** we can now apply the induction hypothesis *)
+  iDestruct "IH" as "-#IH".
+  iSpecialize ("IH" $! (meas - 1)).
+  iAssertSpecialize "IH".
+  { iPureIntro. destruct Hinv', Hinv. rewrite app_length /= in inv_measure1. lia. }
+  iSpecialize ("IH" $! stack marked').
+  iAssertSpecialize "IH" with "[D' D2 D3]".
+  { do 2 iDestruct (diamonds_join with "[$]") as "?"; now rew_qz. }
+  iSpecialize ("IH" with "Ss Sm Sg Pm Ps").
+  Fail wps_apply "IH". (* TODO *)
+  iApply ("IH" with "Vg [Hlocs_hole Pn Sn Hneighbors]").
+  now iApply "Hlocs_hole"; iFrame; auto.
+  iFrame; auto.
+
+  Unshelve.
+  now rewrite replicate_length; lia.
+  now set_solver.
+  now rewrite !fmap_length; lia.
+  exact tt.
+  now rewrite !fmap_length; lia.
+Qed.
+
+(*
+Remarks:
+
+1) iLöb can't be used, because laters are never removed? -> in fact, we can
+
+2) many times, wps_apply "H" results in:
+  Tactic failure: iPoseProof: "H" not found
+
+3) at "let not_empty = vector_size stack", if we don't use wps_bind_nofree, then
+
+  (* TODO: without this mechanism, wps_bind takes a long (infinite?) time *)
+  match goal with |- context [tm_if ?a ?b ?c] => remember (tm_if a b c) as t end.
+  change t with (id t) in Heqt.
+  Opaque id.
+  wps_bind; change (id t) with t in Heqt; subst t.
+  Transparent id.
+  (* solving wps_bind's side obligation more carefully than [set_solver] *)
+  {
+    simpl.
+    repeat
+      match goal with
+      | |- ∅ ⊆ _ => apply empty_subseteq
+      | |- _ ∪ ∅ ⊆ _ => rewrite union_empty_r
+      | |- ∅ ∪ _ ⊆ _ => rewrite union_empty_l
+      | |- _ ∪ _ ⊆ _ => apply union_least
+      | |- locs (subst _ _ _) ⊆ _ => etransitivity; [ now apply locs_subst | ]
+      | |- locs_tm (subst _ _ _) ⊆ _ => etransitivity; [ now apply locs_subst | ]
+      | |- locs (mk_clo ?s ?a ?c) ⊆ ?r => change (locs_tm (mk_clo s a c) ⊆ r); rewrite (locs_mk_clo s a c)
+      | _ => set_solver
+      end.
+  }
+  wps_nofree.
+  wps_apply vector_size_amortized_spec.
+  simpl.
+  rename v0 into nstack.
+  iDestruct select (_ ∗ _)%I as "(%E_nstack & V)".
+*)
